remove dependency on LocalBlockchainTests, fix indentations

execution/tests/ChainPrinters.v
@@ -8,6 +8,8 @@ From ConCert Require Import BoundedN ChainedList.
 
 (* From ConCert.Execution.QCTests Require Import SerializablePrinters. *)
 
+Let Base := TestUtils.LocalChainBase.
+
 (* For monad notations *)
 From ExtLib.Structures Require Import Monads.
 Import MonadNotation. Open Scope monad_scope.
@@ -20,45 +22,39 @@ Import LocalBlockchain.
 Import ListNotations.
 Close Scope address_scope.
 
-Definition AddrSize := (2^8)%N.
-Instance LocalChainBase : ChainBase := TestUtils.LocalChainBase.
-Instance LocalChainBuilder : ChainBuilderType := TestUtils.LocalChainBuilder.
-
 Open Scope list_scope.
 Open Scope string_scope.
 
 Derive Show for positive.
 Derive Show for SerializedType.
 
-Instance showLCB : Show LocalChainBuilder :=
-  {| show a := "LocalChainBuilder{...}" |}.
+Instance showLCB : Show ChainBuilder :=
+  {| show a := "ChainBuilder{...}" |}.
 
-Instance showLocalChainBuilderDepthFirst {n : N} : Show (LocalChainBuilderDepthFirst n) :=
-  {| show a := "LocalChainBuilderDepthFirst{...}" |}.
 
 Instance showChainBuilderType {BaseTypes : ChainBase}: Show (@ChainBuilderType BaseTypes) :=
   {| show a := "ChainBuilderType{...}" |}.
 
-Instance shrinkAmount : Shrink Amount := 
+Instance shrinkAmount : Shrink Amount :=
   {|
     shrink := @shrink Z _
   |}.
 
 Instance showChain (BaseTypes : ChainBase) : Show (@Chain BaseTypes) :=
 {|
-  show c := 
+  show c :=
     let height := show (chain_height c) in
     let slot := show (current_slot c) in
     let fin_height := show (finalized_height c) in
-      "Chain{" ++ "height: "       ++ height     ++ sep 
-                ++ "current slot: " ++ slot       ++ sep 
+      "Chain{" ++ "height: "       ++ height     ++ sep
+                ++ "current slot: " ++ slot       ++ sep
                 ++ "final height: " ++ fin_height ++ "}"
 |}.
 
 Instance showContract {Setup Msg State : Type}
                      `{Serializable Setup}
                      `{Serializable Msg}
-                     `{Serializable State} 
+                     `{Serializable State}
                       : Show (Contract Setup Msg State) :=
 {|
   show c := "Contract{...}"
@@ -66,8 +62,8 @@ Instance showContract {Setup Msg State : Type}
 
 Instance showEnvironment (BaseTypes : ChainBase) `{Show Chain}: Show Environment :=
 {|
-  show env := "Environment{" 
-              ++ "chain: " ++ show (env_chain env) ++ sep 
+  show env := "Environment{"
+              ++ "chain: " ++ show (env_chain env) ++ sep
               ++ "contract states:..."             ++ "}"
 |}.
 
@@ -76,17 +72,17 @@ match st as st0 return interp_type st0 -> string with
   | ser_unit => fun _ => "()"
   | ser_int => fun t => show t
   | ser_bool => fun t => show t
-  | ser_list a => 
-    fun t : list (interp_type a) => 
-      let t_str_list := map (string_of_interp_type a) t in 
-      "[" ++ String.concat ";" t_str_list ++ "]"  
-  | ser_pair a b => 
-    fun t : (interp_type a * interp_type b) => 
-      "(" 
-      ++ string_of_interp_type a (fst t) 
+  | ser_list a =>
+    fun t : list (interp_type a) =>
+      let t_str_list := map (string_of_interp_type a) t in
+      "[" ++ String.concat ";" t_str_list ++ "]"
+  | ser_pair a b =>
+    fun t : (interp_type a * interp_type b) =>
+      "("
+      ++ string_of_interp_type a (fst t)
       ++ ","
       ++ string_of_interp_type b (snd t) ++ ")"
-  end.  
+  end.
 
 Definition ex_serialized_type := ser_pair (ser_list (ser_list ser_bool)) ser_int.
 (* Compute (interp_type ex_serialized_type). *)
@@ -96,18 +92,18 @@ Definition ex_val := ([[true;false];[true;true];[false];[]], 2%Z).
 (* Show and Generator instances for types related to Traces (an execution sequence of contracts on the BC) *)
 Instance showBlockHeader (BaseTypes : ChainBase) `{Show (@Address BaseTypes)} : Show (@BlockHeader BaseTypes) :=
   {|
-    show bh := 
+    show bh :=
       "BlockHeader{" ++ "bheight: "     ++ show (block_height bh)           ++ sep
-                     ++ "bslot: "       ++ show (block_slot bh)             ++ sep 
+                     ++ "bslot: "       ++ show (block_slot bh)             ++ sep
                      ++ "bfin_height: " ++ show (block_finalized_height bh) ++ sep
                      ++ "breward: "     ++ show (block_reward bh)           ++ sep
-                     ++ "bcreator: "    ++ show (block_creator bh)          ++ "}" 
+                     ++ "bcreator: "    ++ show (block_creator bh)          ++ "}"
   |}.
 
   (* We dont show the bound because it may be a very large number which, when converted to nat and then to string, gives a memory overflow. *)
 Instance showBoundedN {bound : N} `{Show N} : Show (BoundedN.BoundedN bound) :=
 {|
-  show bn := match bn with | BoundedN.bounded n _ => show n ++ "%" ++ show bound end  
+  show bn := match bn with | BoundedN.bounded n _ => show n ++ "%" ++ show bound end
 |}.
 
 Instance showBoundedNAddrSize : Show (BoundedN.BoundedN AddrSize) :=
@@ -115,66 +111,66 @@ Instance showBoundedNAddrSize : Show (BoundedN.BoundedN AddrSize) :=
   show := @show (BoundedN.BoundedN AddrSize) showBoundedN
 |}.
 
-Instance showAddress : Show (@Address LocalChainBase) :=
+Instance showAddress : Show (@Address Base) :=
 {|
   show := @show (BoundedN.BoundedN AddrSize) showBoundedNAddrSize
 |}.
 
-Instance showLocalChain : Show (@LocalChain AddrSize) := 
+Instance showLocalChain : Show (@LocalChain AddrSize) :=
 {|
-  show lc := "LocalChain{" 
-              ++ show (lc_height lc) ++ sep 
-              ++ show (lc_slot lc)   ++ sep 
-              ++ show (lc_fin_height lc) 
+  show lc := "LocalChain{"
+              ++ show (lc_height lc) ++ sep
+              ++ show (lc_slot lc)   ++ sep
+              ++ show (lc_fin_height lc)
               ++ sep ++ "... }"
 |}.
 
-Instance showLocalContractCallContext : Show (@ContractCallContext LocalChainBase) :=
+Instance showLocalContractCallContext : Show (@ContractCallContext Base) :=
 {|
 show cctx := "ContractCallContext{"
-             ++ "ctx_from: " ++ show (@ctx_from LocalChainBase cctx) ++ sep
-             ++ "ctx_contract_addr: " ++ show (@ctx_contract_address LocalChainBase cctx) ++ sep
-             ++ "ctx_amount: " ++ show (@ctx_amount LocalChainBase cctx) ++ "}"
+             ++ "ctx_from: " ++ show (@ctx_from Base cctx) ++ sep
+             ++ "ctx_contract_addr: " ++ show (@ctx_contract_address Base cctx) ++ sep
+             ++ "ctx_amount: " ++ show (@ctx_amount Base cctx) ++ "}"
 |}.
 
 Instance showActionBody `{Show SerializedValue} : Show ActionBody :=
 {|
   show a := match a with
-    | act_transfer addr amount => 
-      "(act_transfer " ++ show addr ++ sep ++ show amount ++ ")" 
-    | act_call addr amount ser_value => 
+    | act_transfer addr amount =>
+      "(act_transfer " ++ show addr ++ sep ++ show amount ++ ")"
+    | act_call addr amount ser_value =>
       "(act_call " ++ show addr ++ sep ++ show amount ++ sep ++ show ser_value ++ ")"
     | act_deploy amount contract ser_value =>
       "(act_deploy " ++ show amount ++ sep ++ show ser_value ++ ")"
     end
-|}. 
+|}.
 
-Instance showLocalAction `{Show ActionBody} : Show (@Action LocalChainBase) :=
+Instance showLocalAction `{Show ActionBody} : Show (@Action Base) :=
 {|
   show a := "Action{"
             ++ "act_from: " ++ show (act_from a) ++ sep
             ++ "act_body: " ++ show (act_body a) ++ "}"
-|}. 
+|}.
 
-Instance showLocalActionList `{Show (@Action LocalChainBase)}: Show (list (@Action LocalChainBase)) :=
+Instance showLocalActionList `{Show (@Action Base)}: Show (list (@Action Base)) :=
 {|
   show a := String.concat (";" ++ nl) (map show a)
-|}. 
+|}.
 Existing Instance showLocalActionList | 0.
-Instance showOptLocalActionList `{Show (option (@Action LocalChainBase))}: Show (list (option (@Action LocalChainBase))) :=
+Instance showOptLocalActionList `{Show (option (@Action Base))}: Show (list (option (@Action Base))) :=
 {|
   show a := String.concat (";" ++ nl) (map show a)
-|}. 
+|}.
 Existing Instance showOptLocalActionList | 0.
 
-Instance showChainState : Show (@ChainState LocalChainBase) :=
+Instance showChainState : Show (@ChainState Base) :=
 {|
   show a := "ChainState{" ++ "}"
 |}.
 
 Instance showContractCallInfo {Msg : Type} `{Show Msg} : Show (ContractCallInfo Msg) :=
 {|
-  show info := "ContractCallInfo{" 
+  show info := "ContractCallInfo{"
                 ++ "call_from: " ++ show (call_from info) ++ sep
                 ++ "call_amount: " ++ show (call_amount info) ++ sep
                 ++ "call_msg: " ++ show (call_msg info) ++ sep ++ "}"
