execution/tests/EIP20Tests/EIP20TokenTests.v
@@ -8,13 +8,12 @@ From ConCert Require Import Blockchain.
 From ConCert Require Import LocalBlockchain.
 From ConCert Require Import Serializable.
 From ConCert Require Import BoundedN.
-From ConCert Require Import LocalBlockchainTests.
 From ConCert Require Import Containers.
 From ConCert Require Import EIP20Token.
 Require Import Extras.
 
-From ConCert.Execution.QCTests Require Import 
-	TestUtils ChainPrinters SerializablePrinters EIP20TokenPrinters EIP20TokenGens TraceGens.
+From ConCert.Execution.QCTests Require Import
+  TestUtils ChainPrinters SerializablePrinters EIP20TokenPrinters EIP20TokenGens TraceGens.
 
 (* For monad notations *)
 From ExtLib.Structures Require Import Monads.
@@ -27,13 +26,16 @@ Close Scope address_scope.
 
 (* -------------------------- Tests of the EIP20 Token Implementation -------------------------- *)
 
+Definition Base := TestUtils.LocalChainBase.
+
+
 Definition token_setup := EIP20Token.build_setup creator (100%N).
 Definition deploy_eip20token : @ActionBody Base := create_deployment 0 EIP20Token.contract token_setup.
 
 Let contract_base_addr := BoundedN.of_Z_const AddrSize 128%Z.
 
-Definition chain_with_token_deployed :=  
-  unpack_option (my_add_block lc_initial 
+Definition chain_with_token_deployed :=
+  unpack_option (my_add_block lc_initial
   [
     build_act creator (act_transfer person_1 10);
     build_act creator (act_transfer person_2 10);
@@ -41,26 +43,26 @@ Definition chain_with_token_deployed :=
     build_act creator deploy_eip20token
   ]).
 
-Definition gEIP20TokenChainTraceList max_acts_per_block lc length := 
-  gLocalChainTraceList_fix lc (fun lc _ => 
+Definition gEIP20TokenChainTraceList max_acts_per_block lc length :=
+  gLocalChainTraceList_fix lc (fun lc _ =>
     gEIP20TokenAction lc contract_base_addr) length max_acts_per_block.
 
-Definition token_reachableFrom (lc : LocalChain) pf : Checker := 
+Definition token_reachableFrom (lc : LocalChain) pf : Checker :=
   @reachableFrom AddrSize lc (gEIP20TokenChainTraceList 1) pf.
 
-Definition token_reachableFrom_implies_reachable (lc : LocalChain) pf1 pf2 : Checker := 
+Definition token_reachableFrom_implies_reachable (lc : LocalChain) pf1 pf2 : Checker :=
   reachableFrom_implies_reachable lc (gEIP20TokenChainTraceList 1) pf1 pf2.
 
 Open Scope string_scope.
 Definition debug_gEIP20Checker {A : Type}
                               `{Checkable A}
-                               lc 
+                               lc
                                (act : option Action)
                                : A -> Checker :=
-  whenFail 
+  whenFail
     ("lc balances: " ++ show (lc_account_balances lc) ++ sep ++ nl
     ++ show act
-    ++ "token state: " ++ show (lc_token_contracts_states_deserialized lc) ++ sep ++ nl 
+    ++ "token state: " ++ show (lc_token_contracts_states_deserialized lc) ++ sep ++ nl
     ).
 
 (* Sample (gEIP20TokenAction chain_with_token_deployed contract_base_addr). *)
@@ -80,23 +82,23 @@ Definition msg_is_transfer (cstate : EIP20Token.State) (msg : EIP20Token.Msg) :=
   end.
 
 Definition transfer_balance_update_correct old_state new_state from to tokens :=
-  let get_balance addr state := with_default 0 (FMap.find addr state.(balances)) in 
+  let get_balance addr state := with_default 0 (FMap.find addr state.(balances)) in
   let from_balance_before := get_balance from old_state in
   let to_balance_before := get_balance to old_state in
   let from_balance_after := get_balance from new_state in
   let to_balance_after := get_balance to new_state in
   (* if the transfer is a self-transfer, balances should remain unchained *)
   if address_eqb from to
-  then 
-    (from_balance_before =? from_balance_after) && 
+  then
+    (from_balance_before =? from_balance_after) &&
     (to_balance_before =? to_balance_after)
   else
-    (from_balance_before =? from_balance_after + tokens) && 
+    (from_balance_before =? from_balance_after + tokens) &&
     (to_balance_before + tokens =? to_balance_after).
 
 Definition post_transfer_correct cctx old_state msg (result_opt : option (State * list ActionBody)) :=
   match (result_opt, msg) with
-  | (Some (new_state, _), transfer to tokens) => 
+  | (Some (new_state, _), transfer to tokens) =>
     let from := cctx.(ctx_from) in
     whenFail (show old_state ++ nl ++ show result_opt)
     (checker (transfer_balance_update_correct old_state new_state from to tokens))
@@ -120,7 +122,7 @@ Definition sum_balances_eq_init_supply lc :=
   (* debug_gEIP20Checker lc None *)
   let contract_states := lc_token_contracts_states_deserialized lc in
   checker match FMap.find contract_base_addr contract_states with
-  | Some state => 
+  | Some state =>
     let balances_list := (map snd o FMap.elements) state.(balances) in
     let balances_sum : N := fold_left N.add balances_list 0%N in
     balances_sum =? state.(total_supply)
@@ -136,12 +138,12 @@ Definition sum_balances_eq_init_supply lc :=
 Definition sum_allowances_le_init_supply lc :=
   debug_gEIP20Checker lc None
       (match FMap.find contract_base_addr (lc_token_contracts_states_deserialized lc) with
-      | Some state => 
-        let allowances := map_values_FMap 
+      | Some state =>
+        let allowances := map_values_FMap
           (fun allowance_map => fold_left N.add ((map snd o FMap.elements) allowance_map) 0)
           state.(allowances) in
         let allowances_list := (map snd o FMap.elements) allowances in
-        let allowances_sum := fold_left N.add allowances_list 0%N in 
+        let allowances_sum := fold_left N.add allowances_list 0%N in
         allowances_sum <=? state.(total_supply)
       | None => false
       end).
@@ -149,15 +151,15 @@ Definition sum_allowances_le_init_supply lc :=
 Definition sum_allowances_le_init_supply_P maxLength :=
   forAllTraces maxLength chain_with_token_deployed (gEIP20TokenChainTraceList 2)
     sum_allowances_le_init_supply.
-    
+
 (* QuickChick (sum_allowances_le_init_supply_P 5). *)
 
-Definition person_has_tokens person (n : N) := 
+Definition person_has_tokens person (n : N) :=
   fun lc =>
     match FMap.find contract_base_addr (lc_token_contracts_states_deserialized lc) with
     | Some state => if n =? (FMap_find_ person state.(balances) 0)
                     then Some n
-                    else None  
+                    else None
     | None => None
     end.
 
@@ -168,14 +170,14 @@ Definition person_has_tokens person (n : N) :=
 (* QuickChick (chain_with_token_deployed ~~> person_has_tokens person_3 12). *)
 (* QuickChick (chain_with_token_deployed ~~> person_has_tokens creator 0). *)
 
-(* QuickChick (token_reachableFrom_implies_reachable 
+(* QuickChick (token_reachableFrom_implies_reachable
   chain_with_token_deployed
   (person_has_tokens creator 10)
-  (person_has_tokens creator 0)        
+  (person_has_tokens creator 0)
 ). *)
 
 Notation "'{' lc '~~>' pf1 '===>' pf2 '}'" :=
-  (reachableFrom_implies_tracePropSized_new 3 lc (gEIP20TokenChainTraceList 1) pf1 pf2)   
+  (reachableFrom_implies_tracePropSized_new 3 lc (gEIP20TokenChainTraceList 1) pf1 pf2)
   (at level 90, left associativity).
 
 (* This (false) property says that from the initial chain where the token contract has been deployed,
@@ -183,13 +185,13 @@ Notation "'{' lc '~~>' pf1 '===>' pf2 '}'" :=
    will satisfy that the creator has 10 tokens. This is obviously not true, and QC will give us a counterexample. *)
 (* QuickChick (
   {
-    chain_with_token_deployed 
-    ~~> (person_has_tokens creator 5 o next_lc_of_lcstep) 
+    chain_with_token_deployed
+    ~~> (person_has_tokens creator 5 o next_lc_of_lcstep)
     ===> (fun _ _ post_trace => isSome (person_has_tokens creator 10 (last_state post_trace)))
   }
 ). *)
 
-Definition get_approve_act (act : Action) : option (Address * Address * EIP20Token.Msg) := 
+Definition get_approve_act (act : Action) : option (Address * Address * EIP20Token.Msg) :=
   match act.(act_body) with
   | act_call caddr _ ser_msg =>
     match deserialize EIP20Token.Msg _ ser_msg with
@@ -199,7 +201,7 @@ Definition get_approve_act (act : Action) : option (Address * Address * EIP20Tok
   | _ => None
   end.
 
-Definition get_transferFrom_act (act : Action) : option (Address * Address * EIP20Token.Msg) := 
+Definition get_transferFrom_act (act : Action) : option (Address * Address * EIP20Token.Msg) :=
   match act.(act_body) with
   | act_call caddr _ ser_msg =>
     match deserialize EIP20Token.Msg _ ser_msg with
@@ -209,7 +211,7 @@ Definition get_transferFrom_act (act : Action) : option (Address * Address * EIP
   | _ => None
   end.
 
-Definition state_has_some_approve_act {AddrSize : N} (step : @LocalChainStep AddrSize) := 
+Definition state_has_some_approve_act {AddrSize : N} (step : @LocalChainStep AddrSize) :=
   match step with
   | step_action prev_lc header next_lc acts =>
     match find (isSome o get_approve_act) acts with
@@ -219,8 +221,8 @@ Definition state_has_some_approve_act {AddrSize : N} (step : @LocalChainStep Add
   | _ => None
   end.
 
-Definition delegate_made_no_transferFroms (approve_act_p :  (Address * Address * EIP20Token.Msg)) 
-                                          (trace : list LocalChainStep) := 
+Definition delegate_made_no_transferFroms (approve_act_p :  (Address * Address * EIP20Token.Msg))
+                                          (trace : list LocalChainStep) :=
   let caddr := fst (fst approve_act_p) in
   let approver := snd (fst approve_act_p) in
   match (snd approve_act_p) with
@@ -230,69 +232,69 @@ Definition delegate_made_no_transferFroms (approve_act_p :  (Address * Address *
       let act_not_transferFrom_delegate act :=
         match get_transferFrom_act act with
         | Some (caddr', caller, (transfer_from from to _)) =>
-          if (address_eqb caddr' caddr) 
+          if (address_eqb caddr' caddr)
           then negb ((address_eqb caller delegate) || (address_eqb from approver))
           else true
         | _ => true
         end in
-      forallb act_not_transferFrom_delegate acts  
+      forallb act_not_transferFrom_delegate acts
     ) trace
   | _ => false
   end.
 
-(* Definition forAnyStateInTrace n trace c := 
+(* Definition forAnyStateInTrace n trace c :=
   let trace' := map prev_lc_of_lcstep trace in
   forAll (elems_ chain_with_token_deployed trace') (fun lc =>
   forAllTraces_traceProp n lc (gEIP20TokenChainTraceList 2) c). *)
 
-Definition allower_addr (approve_act_p : (Address * Address * EIP20Token.Msg)) := 
+Definition allower_addr (approve_act_p : (Address * Address * EIP20Token.Msg)) :=
   match snd approve_act_p with
   | (approve _ _ ) => snd (fst approve_act_p)
   | (transfer_from allower _ _) => allower
   | _ => zero_address
   end.
-Definition delegate_addr (approve_act_p : (Address * Address * EIP20Token.Msg)) := 
+Definition delegate_addr (approve_act_p : (Address * Address * EIP20Token.Msg)) :=
   match (snd approve_act_p) with
   | (approve delegate _ ) => Some delegate
   | (transfer_from _ _ _) => Some (snd (fst approve_act_p))
-  | _ => None 
+  | _ => None
   end.
 
-Definition approve_amount (approve_act_p : (Address * Address * EIP20Token.Msg)) := 
+Definition approve_amount (approve_act_p : (Address * Address * EIP20Token.Msg)) :=
   match (snd approve_act_p) with
   | (approve _ amount ) => amount
   | _ => 0
   end.
 
-Definition transfer_from_amount (transferFrom_act_p : (Address * Address * EIP20Token.Msg)) := 
+Definition transfer_from_amount (transferFrom_act_p : (Address * Address * EIP20Token.Msg)) :=
   match (snd transferFrom_act_p) with
   | (transfer_from _ _ amount ) => amount
   | _ => 0
   end.
 
-Definition allower_reapproves_delegate_step allower delegate step := 
+Definition allower_reapproves_delegate_step allower delegate step :=
   let acts := acts_of_lcstep step in
   match find isSome (map get_approve_act acts) with
-  | Some (Some (caddr, caller, (approve delegate' amount)) as act)  =>  
+  | Some (Some (caddr, caller, (approve delegate' amount)) as act)  =>
     if address_eqb caller allower && address_eqb delegate delegate'
     then Some amount
     else None
   | _ => None
   end.
 
-Definition delegate_transferFrom_sum_of_approver approver delegate trace := 
+Definition delegate_transferFrom_sum_of_approver approver delegate trace :=
   fold_left (fun acc step =>
     let transfer_from_acts := fold_left (fun acc act =>
       match get_transferFrom_act act with
       | Some x => x :: acc
       | None => acc
-      end 
+      end
     ) (acts_of_lcstep step) [] in
     let filter_p p := if address_eqb (allower_addr p) approver
                       then match delegate_addr p with
                            | Some delegate' => address_eqb delegate delegate'
                            | None => false
-                           end 
+                           end
                       else false in
     let relevant_transfer_from_acts := filter filter_p transfer_from_acts in
     let step_sum := fold_left (fun acc p => (transfer_from_amount p) + acc) relevant_transfer_from_acts 0 in
@@ -317,9 +319,9 @@ Definition allower_reapproves_transferFrom_correct trace allower delegate (first
     (allower_reapproves_delegate_step allower delegate)
     (fun new_approval_amount pre_trace _ =>
       let trace_until_reapproval := app trace (removelast pre_trace) in
-      let delegate_spent_until_reapproval := delegate_transferFrom_sum_of_approver allower delegate trace_until_reapproval in 
-      let delegate_spent_incl_reapproval_act := 
-        delegate_transferFrom_sum_of_approver allower delegate (trace ++ pre_trace) in 
+      let delegate_spent_until_reapproval := delegate_transferFrom_sum_of_approver allower delegate trace_until_reapproval in
+      let delegate_spent_incl_reapproval_act :=
+        delegate_transferFrom_sum_of_approver allower delegate (trace ++ pre_trace) in
       let total_allowed := delegate_spent_until_reapproval + new_approval_amount in
       (new_approval_amount <? first_approval_amount) ==>
       whenFail (show delegate ++ " spent "
@@ -327,11 +329,11 @@ Definition allower_reapproves_transferFrom_correct trace allower delegate (first
         ++ " on behalf of " ++ show allower
         ++ " when they were only allowed to spend at most "
         ++ show total_allowed  ++ nl)
-      (delegate_spent_incl_reapproval_act <=? total_allowed) 
+      (delegate_spent_incl_reapproval_act <=? total_allowed)
     )
   end.
 
-Definition reapprove_transfer_from_safe_P := 
+Definition reapprove_transfer_from_safe_P :=
   (reachableFrom_implies_tracePropSized_new 3 chain_with_token_deployed (gEIP20TokenChainTraceList 2))
   state_has_some_approve_act
   (fun approve_act_p pre_trace post_trace =>
@@ -340,14 +342,14 @@ Definition reapprove_transfer_from_safe_P :=
       allower_reapproves_transferFrom_correct post_trace
                                               (allower_addr approve_act_p)
                                               delegate
-                                              (approve_amount approve_act_p)     
-      ) 
+                                              (approve_amount approve_act_p)
+      )
     (* ) *)
   ).
 
 (* QuickChick reapprove_transfer_from_safe_P. *)
 
-(* coqtop-stdout:Begin Trace: 
+(* coqtop-stdout:Begin Trace:
 
 coqtop-stdout:step_action{Action{act_from: 10%256, act_body: (act_call 128%256, 0, transfer_from 12%256 12%256 7)};
 
