execution/tests/TraceGens.v
@@ -1,13 +1,13 @@
-(* 
+(*
   The ChainTrace datatype is defined as a ChainedList of ChainStates and ChainSteps.
   The ChainStep is an inductive relation with constructors 'step_block', 'step_action', and 'step_permute'.
   Each constructor is guarded with a number of propositions, requiring various validity conditions.
-  
+
   This makes it hard to construct a generator for the ChainTrace type, so instead we initially construct a simpler model
   for chain traces, which is essentially just a list of chain states.
   But since we are working in the context of black-box testing, this may even be a better approach than trying to implement
   generators for the ChainTrace type, since we don't want to ensure/require that certain conditions hold, we only want
-  to generate data from the given functions, and see what result we get. 
+  to generate data from the given functions, and see what result we get.
 *)
 
 Global Set Warnings "-extraction-logical-axiom".
@@ -19,7 +19,6 @@ From ConCert Require Import Blockchain.
 From ConCert Require Import LocalBlockchain.
 From ConCert Require Import Serializable.
 From ConCert Require Import BoundedN.
-From ConCert Require Import LocalBlockchainTests.
 From ConCert Require Import Containers.
 From ConCert Require Import ResultMonad.
 Require Import Extras.
@@ -37,9 +36,17 @@ Import BoundedN.Stdpp.
 Import LocalBlockchain.
 Import ListNotations.
 Close Scope address_scope.
-Definition AddrSize := (2^8)%N.
 
 Definition LocalChainBase : ChainBase := TestUtils.LocalChainBase.
+
+Definition add_block (chain : ChainBuilder) acts : result ChainBuilder AddBlockError :=
+  let header :=
+      {| block_height := S (chain_height chain);
+         block_slot := S (current_slot chain);
+         block_finalized_height := finalized_height chain;
+         block_creator := creator;
+         block_reward := 50; |} in
+  builder_add_block chain header acts.
 
 Definition next_header (chain : ChainBuilder) :=
     {| block_height := S (chain_height chain);
@@ -48,7 +55,7 @@ Definition next_header (chain : ChainBuilder) :=
        block_creator := creator;
        block_reward := 50; |}.
 
-Definition next_header_lc (chain : @LocalChain AddrSize) :=
+Definition next_header_lc (chain : @LocalChain AddrSize)  :=
     {| block_height := S (chain_height chain);
        block_slot := S (current_slot chain);
        block_finalized_height := finalized_height chain;
@@ -56,7 +63,7 @@ Definition next_header_lc (chain : @LocalChain AddrSize) :=
        block_reward := 50; |}.
 
 (* Adds a new block with a given list of actions in that block. Uses next_header_lc to compute header info. *)
-Definition my_add_block c acts := 
+Definition my_add_block c acts :=
   match (add_block_exec true c (next_header_lc c) acts) with
   | Err _ => None
   | Ok r => Some r
@@ -67,14 +74,14 @@ Definition my_add_block c acts :=
    A step can either add an empty new block, or add a new block with some actions to execute.
    The next_chain is assumed to be related to prev_chain with the 'my_add_block' function *)
 Inductive LocalChainStep {AddrSize : N} : Type :=
-| step_add_block : forall (prev_chain : @LocalChain AddrSize) 
-                          (header : BlockHeader) 
+| step_add_block : forall (prev_chain : @LocalChain AddrSize)
+                          (header : BlockHeader)
                           (next_chain : @LocalChain AddrSize), LocalChainStep
-| step_action : forall (prev_chain : @LocalChain AddrSize) 
-                       (header : BlockHeader) 
-                       (next_chain : @LocalChain AddrSize) 
+| step_action : forall (prev_chain : @LocalChain AddrSize)
+                       (header : BlockHeader)
+                       (next_chain : @LocalChain AddrSize)
                        (acts : list Action), LocalChainStep.
-                  
+
 (* Helper functions *)
 
 Definition acts_of_lcstep (state : @LocalChainStep AddrSize) :=
@@ -82,7 +89,7 @@ Definition acts_of_lcstep (state : @LocalChainStep AddrSize) :=
   | step_add_block _ _ _ => []
   | step_action _ _ _ acts => acts
   end.
-                       
+
 Definition prev_lc_of_lcstep (state : @LocalChainStep AddrSize) :=
   match state with
   | step_add_block prev _ _ => prev
@@ -97,13 +104,13 @@ Definition next_lc_of_lcstep (state : @LocalChainStep AddrSize) : LocalChain :=
 Close Scope string_scope.
 
 (* Shallow Equality of LocalChains *)
-Definition lc_shallow_eqb lc1 lc2 : bool := 
-  (lc_height lc1 =? lc_height lc2) 
-  && (lc_slot lc1 =? lc_slot lc2) 
+Definition lc_shallow_eqb lc1 lc2 : bool :=
+  (lc_height lc1 =? lc_height lc2)
+  && (lc_slot lc1 =? lc_slot lc2)
   && (@lc_fin_height AddrSize lc1 =? @lc_fin_height AddrSize lc2).
 
 
-Definition mk_basic_step_add_block c : option (LocalChain * LocalChainStep) := 
+Definition mk_basic_step_add_block c : option (LocalChain * LocalChainStep) :=
   let header := (next_header_lc c) in
   let next := add_block_exec true c header [] in
   match next with
@@ -111,7 +118,7 @@ Definition mk_basic_step_add_block c : option (LocalChain * LocalChainStep) :=
   | Ok c_next => Some (c_next, step_add_block c header c_next)
   end.
 
-Definition mk_basic_step_action c acts : option (LocalChain * LocalChainStep) := 
+Definition mk_basic_step_action c acts : option (LocalChain * LocalChainStep) :=
   let header := (next_header_lc c) in
   let next := add_block_exec true c header acts in
   match next with
@@ -123,8 +130,8 @@ Open Scope string_scope.
 Instance showLocalChainStepVerbose {AddrSize : N} `{Show (@LocalChain AddrSize)} : Show (@LocalChainStep AddrSize) :=
 {|
   show step := match step with
-  | step_add_block prev header next => 
-    "step_add_block{ prev_lc: " ++ show prev ++ sep ++ "header: " ++ show header ++ sep ++ "next_lc:" ++ show next ++ "}"  
+  | step_add_block prev header next =>
+    "step_add_block{ prev_lc: " ++ show prev ++ sep ++ "header: " ++ show header ++ sep ++ "next_lc:" ++ show next ++ "}"
   | step_action prev header next acts =>
     "step_action{ prev_lc: " ++ show prev ++ sep ++ "header: " ++ show header ++ sep ++ "next_lc:" ++ show next ++ sep ++ "acts: " ++ show acts ++ "}"
   end
@@ -133,8 +140,8 @@ Instance showLocalChainStepVerbose {AddrSize : N} `{Show (@LocalChain AddrSize)}
 Instance showLocalChainStep {AddrSize : N} `{Show (@LocalChain AddrSize)} : Show (@LocalChainStep AddrSize) :=
 {|
   show step := match step with
-  | step_add_block prev header next => 
-    "step_add_block{ ... }"  
+  | step_add_block prev header next =>
+    "step_add_block{ ... }"
   | step_action prev header next acts =>
     "step_action{" ++ show acts ++ "}"
   end
@@ -148,13 +155,13 @@ Definition LocalChainTraceList {AddrSize : N} := list (@LocalChainStep AddrSize)
 Fixpoint gLocalChainTraceList_fix (prev_lc : LocalChain)
                               (gActOptFromLCSized : LocalChain -> nat -> G (option Action))
                               (length : nat)
-                              (max_nr_acts_per_block : nat) 
+                              (max_nr_acts_per_block : nat)
                               : G LocalChainTraceList :=
   match length with
   | 0 => returnGen []
-  | S length => 
+  | S length =>
     lc_opt <- backtrack [
-      (10, 
+      (10,
           (* What we're essentially doing here trying twice and then discarding one - to increase robustness.  *)
           let try_twice g := backtrack [(1, g);(1, g)] in
           try_twice (
@@ -176,7 +183,7 @@ Fixpoint gLocalChainTraceList_fix (prev_lc : LocalChain)
       (* (3, liftM (mk_basic_step_action prev_lc ) (optToVector 1 (gDeployCongressActionFromLC prev_lc)))  *)
       ] ;;
     match lc_opt with
-          | Some (lc, step) => 
+          | Some (lc, step) =>
             trace <- (gLocalChainTraceList_fix lc gActOptFromLCSized length max_nr_acts_per_block) ;;
             match trace with
             | [] => returnGen [step]
@@ -191,7 +198,7 @@ Instance showLocalChainList : Show LocalChainTraceList :=
 {|
   show l := nl ++ "Begin Trace: " ++ nl ++ String.concat (";;" ++ nl) (map show l) ++ nl ++ "End Trace"
 |}.
-Close Scope string_scope.  
+Close Scope string_scope.
 
 (* -------------------- Checker combinators on traces --------------------  *)
 
@@ -204,11 +211,11 @@ Definition forAllTraces {prop : Type}
                         (gTrace : LocalChain -> nat -> G LocalChainTraceList)
                         (pf : LocalChain -> prop)
                         : Checker :=
-  forAll (gTrace init_lc maxLength) 
+  forAll (gTrace init_lc maxLength)
   (fun trace => match trace with
                 | [] => false ==> true
                 | _ => conjoin (map (checker o pf o next_lc_of_lcstep) trace)
-                end).   
+                end).
 
 (* A variant where the property is over the step *)
 Definition forAllTraces_stepProp {prop : Type}
@@ -219,11 +226,11 @@ Definition forAllTraces_stepProp {prop : Type}
                         (gTrace : LocalChain -> nat -> G LocalChainTraceList)
                         (pf : LocalChainStep -> prop)
                         : Checker :=
-  forAll (gTrace init_lc maxLength) 
+  forAll (gTrace init_lc maxLength)
   (fun trace => match trace with
                 | [] => false ==> true
                 | _ => conjoin (map (checker o pf) trace)
-                end).  
+                end).
 
 (* A variant where the property is over the whole trace *)
 Definition forAllTraces_traceProp {prop : Type}
@@ -237,20 +244,20 @@ Definition forAllTraces_traceProp {prop : Type}
   forAll (gTrace init_lc maxLength)  pf.
 
 Definition reachableFromSized {AddrSize : N}
-                         (maxLength : nat) 
+                         (maxLength : nat)
                          (init_lc : LocalChain)
                          (gTrace : (@LocalChain AddrSize) -> nat -> G LocalChainTraceList)
                          (pf : LocalChainStep -> bool)
-                         : Checker := 
+                         : Checker :=
   existsP (gTrace init_lc maxLength) (fun trace => existsb pf trace).
 
-Definition reachableFrom {AddrSize : N} init_lc gTrace pf : Checker := 
+Definition reachableFrom {AddrSize : N} init_lc gTrace pf : Checker :=
   sized (fun n => @reachableFromSized AddrSize n init_lc gTrace pf).
 
 Fixpoint cut_at_first_satisfying_fix {A : Type} (p : A -> bool) (l : list A) (acc : list A) : option (list A) :=
   match l with
   | [] => None
-  | x::xs => if p x 
+  | x::xs => if p x
              then Some (acc ++ [x])
              else (cut_at_first_satisfying_fix p xs (acc ++ [x]))
   end.
@@ -260,52 +267,52 @@ Definition cut_at_first_satisfying_ {A : Type} (p : A -> bool) (l : list A) := c
 (* represents: if there is a state x, satisfying pf1, reachable from init_lc,
                then there is a state y, satisfyring pf2, reachable from state x. *)
 Definition reachableFrom_implies_reachableSized
-                         (maxLength : nat) 
+                         (maxLength : nat)
                          (init_lc : (@LocalChain AddrSize))
                          (gTrace : @LocalChain AddrSize -> nat -> G (list (@LocalChainStep AddrSize)))
                          (pf1 : LocalChain -> bool)
                          (pf2 : LocalChain -> bool)
-                         : Checker := 
-  expectFailure (forAll (gTrace init_lc maxLength)  
+                         : Checker :=
+  expectFailure (forAll (gTrace init_lc maxLength)
     (fun trace =>
      match cut_at_first_satisfying_ (pf1 o next_lc_of_lcstep) trace with
       | None => checker true
-      | Some trace_cut => 
+      | Some trace_cut =>
         let new_init_lc := (List.last (map next_lc_of_lcstep trace_cut) init_lc) in
-        expectFailure (forAll (gTrace new_init_lc maxLength) 
-        (fun new_trace => whenFail 
+        expectFailure (forAll (gTrace new_init_lc maxLength)
+        (fun new_trace => whenFail
           ("Success - found witnesses satisfying the predicates:" ++ nl ++
           "First trace:"  ++
-          show trace_cut ++ nl ++ 
+          show trace_cut ++ nl ++
           "Second trace:" ++
           show new_trace ++ nl)
           ((checker o negb) (existsb pf2 (map (next_lc_of_lcstep) new_trace)))
         ))
       end)).
 
-Definition reachableFrom_implies_reachable init_lc gTrace pf1 pf2 : Checker := 
+Definition reachableFrom_implies_reachable init_lc gTrace pf1 pf2 : Checker :=
   sized (fun n => reachableFrom_implies_reachableSized n init_lc gTrace pf1 pf2).
 
 (* If a state satisfying pf1 is reachable from init_lc, then any trace from this state satisfies pf_trace  *)
 Definition reachableFrom_implies_tracePropSized
                          {A prop : Type}
                         `{Checkable prop}
-                         (maxLength : nat) 
+                         (maxLength : nat)
                          (init_lc : (@LocalChain AddrSize))
                          (gTrace : @LocalChain AddrSize -> nat -> G (list (@LocalChainStep AddrSize)))
                          (pf1 : LocalChainStep -> option A)
                          (pf_trace : A -> LocalChainTraceList -> prop)
-                         : Checker := 
-  forAll (gTrace init_lc maxLength)  
+                         : Checker :=
+  forAll (gTrace init_lc maxLength)
   (fun trace =>
-    let pf1_bool lc := match pf1 lc with Some _ => true | None => false end in 
+    let pf1_bool lc := match pf1 lc with Some _ => true | None => false end in
     match cut_at_first_satisfying_ pf1_bool trace with
-    | Some (x::xs as trace_cut) => 
+    | Some (x::xs as trace_cut) =>
       let last_step := (List.last trace_cut x) in
       isSomeCheck (pf1 last_step)
         (fun a =>
           let new_init_lc := next_lc_of_lcstep last_step in
-          (forAll (gTrace new_init_lc maxLength) 
+          (forAll (gTrace new_init_lc maxLength)
             (fun new_trace => (pf_trace a new_trace))
           )
         )
@@ -318,13 +325,13 @@ Definition reachableFrom_implies_traceProp {A : Type}
                                            (gTrace : @LocalChain AddrSize -> nat -> G (list (@LocalChainStep AddrSize)))
                                            (pf1 : LocalChainStep -> option A)
                                            (pf_trace : A -> LocalChainTraceList -> bool)
-                                           : Checker := 
+                                           : Checker :=
   sized (fun n => reachableFrom_implies_tracePropSized n init_lc gTrace pf1 pf_trace).
 
 Fixpoint split_at_first_satisfying_fix {A : Type} (p : A -> bool) (l : list A) (acc : list A) : option (list A * list A) :=
   match l with
   | [] => None
-  | x::xs => if p x 
+  | x::xs => if p x
              then Some (acc ++ [x], xs)
              else (split_at_first_satisfying_fix p xs (acc ++ [x]))
   end.
@@ -337,25 +344,25 @@ Definition split_at_first_satisfying {A : Type} (p : A -> bool) (l : list A) : o
 Definition reachableFrom_implies_tracePropSized_new
                          {A prop : Type}
                         `{Checkable prop}
-                         (maxLength : nat) 
+                         (maxLength : nat)
                          (init_lc : (@LocalChain AddrSize))
                          (gTrace : @LocalChain AddrSize -> nat -> G (list (@LocalChainStep AddrSize)))
                          (pf1 : LocalChainStep -> option A)
                          (pf_trace : A -> LocalChainTraceList -> LocalChainTraceList -> prop)
-                         : Checker := 
-  forAll (gTrace init_lc maxLength) 
+                         : Checker :=
+  forAll (gTrace init_lc maxLength)
   (fun trace =>
-    let pf1_bool := isSome o pf1 in 
+    let pf1_bool := isSome o pf1 in
     match split_at_first_satisfying pf1_bool trace with
     | Some ((x::xs) as pre, (y::ys) as post) =>
       let last_step := (List.last pre x) in
-      isSomeCheck (pf1 last_step) 
+      isSomeCheck (pf1 last_step)
         (fun a => (pf_trace a pre post))
     | _ => false ==> true
     end).
 
 (* if pre tests true, then post tests true, for all tested execution traces *)
-Definition pre_post_assertion {Setup Msg State prop : Type} 
+Definition pre_post_assertion {Setup Msg State prop : Type}
                              `{Checkable prop}
                              `{Serializable Msg}
                              `{Serializable State}
@@ -386,24 +393,20 @@ Definition pre_post_assertion {Setup Msg State prop : Type}
       let msgs := messages_of_step step in
       let contracts := contracts_of_step step in
       let execute_receive chain caddr cstate act msg :=
-        let amount := 
+        let amount :=
           match act.(act_body) with
           | act_call _ amount _ => amount
           | _ => 0%Z
-          end in 
+          end in
         let cctx := build_ctx act.(act_from) caddr amount in
         let new_state := c.(receive) chain cctx cstate (Some msg) in
         (cctx, new_state) in
 
-      conjoin (map (fun p =>
-        let caddr := fst p in
-        let cstate := snd p in
+      conjoin (map (fun '(caddr, cstate) =>
         (* test that executing receive on the messages that satisfy the precondition, also satisfy the postcondition *)
-        conjoin (map (fun msg_act_pair =>
-          let msg := snd msg_act_pair in
-          let act := fst msg_act_pair in
-          let (cctx, post_state) := execute_receive lc caddr cstate act msg in 
-          pre cstate msg ==> post cctx cstate msg post_state 
+        conjoin (map (fun '(act, msg) =>
+          let (cctx, post_state) := execute_receive lc caddr cstate act msg in
+          pre cstate msg ==> post cctx cstate msg post_state
         ) msgs)
       ) contracts) in
     (* combine it all with the forAllTraces checker combinator *)
