execution/tests/CongressTests/CongressGens.v
@@ -34,37 +34,37 @@ Definition genToOpt {A : Type} (g : G A) : G (option A) :=
 Definition gRulesSized (n : nat) : G Rules :=
   vote_count <- choose(1%Z, 1000%Z) ;;
   margin <- choose(1%Z, 1000%Z) ;;
-  liftM (build_rules vote_count margin) arbitrary.  
+  liftM (build_rules vote_count margin) arbitrary.
 
 Instance genRulesSized : GenSized Rules :=
 {|
   arbitrarySized := gRulesSized
 |}.
 
-Instance genSetupSized : GenSized Setup := 
+Instance genSetupSized : GenSized Setup :=
 {|
   arbitrarySized n := liftM build_setup (arbitrarySized n)
 |}.
-  
+
 (* generators of actions from the LocalChain context type *)
 
-Definition allProposalsOfLC lc : FMap ProposalId Proposal := 
+Definition allProposalsOfLC lc : FMap ProposalId Proposal :=
   let all_states := FMap.values (lc_contract_state_deserialized Congress.State lc) in
   let proposals_list : list (ProposalId * Proposal):= fold_left (fun acc s => FMap.elements (proposals s) ++ acc ) all_states [] in
   FMap.of_list proposals_list.
 
 Definition allProposalsWithVotes lc : FMap ProposalId Proposal :=
- filter_FMap (fun p => 0 <? FMap.size (votes (snd p))) (allProposalsOfLC lc).
+ filter_FMap (fun '(_, p) => 0 <? FMap.size (votes p)) (allProposalsOfLC lc).
 
-Definition congressContractsMembers lc : FMap Address (list Address) := 
+Definition congressContractsMembers lc : FMap Address (list Address) :=
  map_values_FMap (fun state => map fst (FMap.elements (members state))) (lc_contract_state_deserialized Congress.State lc).
 
- Definition congressContractsMembers_nonempty lc : FMap Address (list Address) := 
- let members_map := 
+ Definition congressContractsMembers_nonempty lc : FMap Address (list Address) :=
+ let members_map :=
   map_values_FMap (fun state => map fst (FMap.elements (members state))) (lc_contract_state_deserialized Congress.State lc) in
-  filter_FMap (fun p => 0 <? length (snd p)) members_map. 
+  filter_FMap (fun p => 0 <? length (snd p)) members_map.
 
-Definition congressContractsMembers_nonempty_nonowners lc : FMap Address (list Address) :=   
+Definition congressContractsMembers_nonempty_nonowners lc : FMap Address (list Address) :=
   map_filter_FMap (fun p =>
     let contract_addr := fst p in
     let state := snd p in
@@ -73,24 +73,24 @@ Definition congressContractsMembers_nonempty_nonowners lc : FMap Address (list A
     if 0 <? length non_owner_members then Some non_owner_members else None
   ) (lc_contract_state_deserialized Congress.State lc).
 
-Definition gCongressMember (lc : LocalChain) 
-                           (contract_addr : Address) 
-                           : G (option Address) := 
+Definition gCongressMember (lc : LocalChain)
+                           (contract_addr : Address)
+                           : G (option Address) :=
   let members_map := (congressContractsMembers lc) in
   bindGenOpt (returnGen (FMap.find contract_addr members_map))
-  (fun members => 
+  (fun members =>
     match members with
     | [] => returnGen None
     | m::ms => liftM Some (elems_ m members)
     end).
 
-Definition gCongressMember_without_caller (lc : LocalChain) 
-                           (calling_addr : Address) 
-                           (contract_addr : Address) 
-                           : G (option Address) := 
+Definition gCongressMember_without_caller (lc : LocalChain)
+                           (calling_addr : Address)
+                           (contract_addr : Address)
+                           : G (option Address) :=
   let members_map := (congressContractsMembers lc) in
   bindGenOpt (returnGen (FMap.find contract_addr members_map))
-  (fun members => 
+  (fun members =>
     let members_without_caller := List.remove address_eqdec calling_addr members in
     match members_without_caller with
     | [] => returnGen None
@@ -109,23 +109,23 @@ Fixpoint try_newCongressMember_fix (members : list Address) nr_attempts curr_nr 
             end
   end in aux nr_attempts curr_nr.
 
-  
+
 Definition try_newCongressMember (lc : LocalChain)
-                                 (congress_addr : Address) 
-                                 (nr_attempts : nat) : option Address := 
+                                 (congress_addr : Address)
+                                 (nr_attempts : nat) : option Address :=
   let current_members_opt := FMap.find congress_addr (congressContractsMembers lc) in
   match current_members_opt with
   | Some current_members => try_newCongressMember_fix current_members nr_attempts 0
   | None => None
   end.
 
-Definition bindCallerIsOwnerOpt {A : Type} 
-                                (lc : LocalChain) 
+Definition bindCallerIsOwnerOpt {A : Type}
+                                (lc : LocalChain)
                                 (calling_addr : Address)
                                 (contract_addr : Address)
-                                (g : G (option A)) : G (option A) := 
-  if address_eqb calling_addr contract_addr 
-  then g 
+                                (g : G (option A)) : G (option A) :=
+  if address_eqb calling_addr contract_addr
+  then g
   else let owner_opt := FMap.find contract_addr (lc_contract_owners lc) in
   match owner_opt with
   | None => returnGen None
@@ -134,11 +134,11 @@ Definition bindCallerIsOwnerOpt {A : Type}
                   else returnGen None
   end.
 
-Definition try_gNewOwner lc calling_addr contract_addr : G (option Address):= 
+Definition try_gNewOwner lc calling_addr contract_addr : G (option Address):=
   bindCallerIsOwnerOpt lc calling_addr contract_addr (gCongressMember_without_caller lc calling_addr contract_addr).
 
 (* Sample (@gMsgSimpleFromLC lc_initial). *)
-(* 
+(*
 Definition optToList {A : Type} : (G (option A)) -> G (list A) :=
   fun g =>
   l <- listOf g ;;
@@ -148,9 +148,9 @@ Definition optToList {A : Type} : (G (option A)) -> G (list A) :=
                           end) l []
   in returnGen l'. *)
 
-Definition vote_proposal (contract_members_and_proposals : FMap Address (FMap Address (list ProposalId))) 
+Definition vote_proposal (contract_members_and_proposals : FMap Address (FMap Address (list ProposalId)))
                          (mk_call : Address -> Address -> Msg -> G (option Action))
-                         (vote : ProposalId -> Msg):= 
+                         (vote : ProposalId -> Msg):=
   p <- sampleFMapOpt contract_members_and_proposals ;;
   let contract_addr := fst p in
   let members_and_proposals := snd p in
@@ -162,8 +162,8 @@ Definition vote_proposal (contract_members_and_proposals : FMap Address (FMap Ad
 
 (* Returns a mapping to proposals which have been discussed long enough, according to the
    current rules in the given LocalChain *)
-Definition finishable_proposals (lc : LocalChain) 
-                                : FMap Address (FMap ProposalId Proposal) := 
+Definition finishable_proposals (lc : LocalChain)
+                                : FMap Address (FMap ProposalId Proposal) :=
   let contracts_rules : FMap Address Rules := map_values_FMap state_rules (lc_contract_state_deserialized Congress.State lc) in
   map_filter_FMap (fun p =>
     let caddr := fst p in
@@ -171,7 +171,7 @@ Definition finishable_proposals (lc : LocalChain)
     match FMap.find caddr contracts_rules with
     | Some rules =>
       let pids_map_filtered := filter_FMap (fun p =>
-        (snd p).(proposed_in) + rules.(debating_period_in_blocks) <=? lc.(lc_slot)  
+        (snd p).(proposed_in) + rules.(debating_period_in_blocks) <=? lc.(lc_slot)
       ) pids_map in
       if 0 <? FMap.size pids_map_filtered
       then Some pids_map_filtered
@@ -182,15 +182,15 @@ Definition finishable_proposals (lc : LocalChain)
 .
 
 Fixpoint gCongressActionNew (lc : LocalChain) (fuel : nat) : G (option Action) :=
-  let mk_call contract_addr caller_addr msg := 
+  let mk_call contract_addr caller_addr msg :=
     amount <- match lc_account_balance lc caller_addr with
               | Some caller_balance => genToOpt (choose (0%Z, caller_balance))
               | None => returnGenSome 0%Z
               end ;;
-    returnGenSome (build_act caller_addr 
+    returnGenSome (build_act caller_addr
       (congress_action_to_chain_action (cact_call contract_addr amount (serializeMsg msg)))) in
   match fuel with
-  | 0 => 
+  | 0 =>
     let proposals_map := allProposalsOfLC lc in
     let proposals_with_votes := allProposalsWithVotes lc in
     (* let bindCallerIsOwner {T : Type} := @bindCallerIsOwnerOpt T lc calling_addr contract_addr in *)
@@ -203,16 +203,16 @@ Fixpoint gCongressActionNew (lc : LocalChain) (fuel : nat) : G (option Action) :
           match owner_opt with
           | Some owner_addr =>
             new_owner <- (try_gNewOwner lc owner_addr contract_addr) ;;
-            mk_call contract_addr owner_addr (transfer_ownership new_owner) 
+            mk_call contract_addr owner_addr (transfer_ownership new_owner)
           | None => returnGen None
           end
-      ) ; 
+      ) ;
       (* change_rules *)
       (1, p <- sampleFMapOpt (lc_contract_owners lc) ;;
           let contract_addr := fst p in
           let owner_addr := snd p in
           rules <- genToOpt (gRulesSized 4) ;;
-          (mk_call contract_addr owner_addr (change_rules rules)) 
+          (mk_call contract_addr owner_addr (change_rules rules))
       ) ;
       (* add_member *)
       (2, p <- sampleFMapOpt (lc_contract_owners lc) ;;
@@ -231,7 +231,7 @@ Fixpoint gCongressActionNew (lc : LocalChain) (fuel : nat) : G (option Action) :
           let owner_opt := FMap.find contract_addr (lc_contract_owners lc) in
           match owner_opt with
           | Some owner_addr =>
-            mk_call contract_addr owner_addr (remove_member member)        
+            mk_call contract_addr owner_addr (remove_member member)
           | None => returnGen None
           end
       ) ;
@@ -239,22 +239,22 @@ Fixpoint gCongressActionNew (lc : LocalChain) (fuel : nat) : G (option Action) :
       (* Requirements:
          - contract with a proposal and members must exist
          - only members which have not already voted can vote again *)
-      (2, vote_proposal (lc_contract_members_and_proposals_new_voters lc) 
+      (2, vote_proposal (lc_contract_members_and_proposals_new_voters lc)
                         mk_call vote_for_proposal ) ;
       (* vote_against_proposal *)
-      (2, vote_proposal (lc_contract_members_and_proposals_new_voters lc) 
+      (2, vote_proposal (lc_contract_members_and_proposals_new_voters lc)
                         mk_call vote_against_proposal ) ;
       (* retract_vote *)
-      (2, vote_proposal (lc_contract_members_and_proposals_with_votes lc) 
+      (2, vote_proposal (lc_contract_members_and_proposals_with_votes lc)
                         mk_call retract_vote) ;
       (* finish_proposal *)
       (* Requirements:
          - only contract owner can finish proposals
          - the debating period must have passed *)
-      (2, p <- sampleFMapOpt (finishable_proposals lc) ;; 
+      (2, p <- sampleFMapOpt (finishable_proposals lc) ;;
         let contract_addr := fst p in
         match FMap.find contract_addr (lc_contract_owners lc) with
-        | Some owner_addr => 
+        | Some owner_addr =>
           p' <- sampleFMapOpt (snd p) ;;
           let pid := fst p' in
           mk_call contract_addr owner_addr (finish_proposal pid)
@@ -264,7 +264,7 @@ Fixpoint gCongressActionNew (lc : LocalChain) (fuel : nat) : G (option Action) :
   | S fuel' => backtrack [
     (1, gCongressActionNew lc fuel') ;
     (* add_proposal *)
-    (1, 
+    (1,
       (* recurse. Msg is converted to a SerializedType using 'serialize' *)
       (* This makes it possible to create proposals about proposals about proposals etc... *)
       (* TODO: currently we don't support having multiple actions in a proposal *)
@@ -274,16 +274,16 @@ Fixpoint gCongressActionNew (lc : LocalChain) (fuel : nat) : G (option Action) :
       act <- gCongressActionNew lc fuel' ;;
       let caller_addr := act.(act_from) in
       match act.(act_body) with
-      | act_call contract_addr amount msg => 
+      | act_call contract_addr amount msg =>
         member <- gCongressMember lc contract_addr ;;
-        let ca := cact_call contract_addr amount msg in  
+        let ca := cact_call contract_addr amount msg in
         mk_call contract_addr member (create_proposal [ca])
       | _ => returnGenSome act
       end)
-  ] 
+  ]
   end.
 
-Definition gDeployCongressActionFromLC lc : G (option Action) := 
+Definition gDeployCongressActionFromLC lc : G (option Action) :=
   calling_addr_opt <- gAccountAddrFromLocalChain lc ;;
   setup <- arbitrary ;;
   deploy_act <- (gDeploymentAction Congress.contract setup) ;;
