execution/tests/CongressTests/CongressTests.v
@@ -1,10 +1,9 @@
 From ConCert Require Import Blockchain LocalBlockchain Congress.
 From ConCert Require Import Serializable.
-From ConCert Require Import LocalBlockchainTests.
 From ConCert Require Import BoundedN ChainedList.
 Require Import Extras.
 
-From ConCert.Execution.QCTests Require Import 
+From ConCert.Execution.QCTests Require Import
   TestUtils ChainPrinters CongressGens CongressPrinters SerializablePrinters TraceGens.
 
 Require Import ZArith Strings.Ascii Strings.String.
@@ -23,27 +22,78 @@ Notation "f 'o' g" := (compose f g) (at level 50).
 
 Definition LocalChainBase : ChainBase := TestUtils.LocalChainBase.
 
+
+(* chains for deploying congress with some existing members *)
+Definition chain1 : ChainBuilder := builder_initial.
+
+(* Creator created an empty block (and gets some coins) *)
+Definition chain2 : ChainBuilder :=
+  unpack_result (add_block chain1 []).
+
+(* Creator transfers 10 coins to person_1 *)
+Definition chain3 : ChainBuilder :=
+  unpack_result (add_block chain2 [build_act creator (act_transfer person_1 10)]).
+
+Definition setup_rules :=
+  {| min_vote_count_permille := 200; (* 20% of congress needs to vote *)
+      margin_needed_permille := 501;
+      debating_period_in_blocks := 0; |}.
+
+Definition setup := Congress.build_setup setup_rules.
+Definition deploy_congress : ActionBody :=
+  create_deployment 5 Congress.contract setup.
+Definition chain4 : ChainBuilder :=
+  unpack_result (add_block chain3 [build_act person_1 deploy_congress]).
+Definition congress_1 : Address :=
+  match outgoing_txs (builder_trace chain4) person_1 with
+  | tx :: _ => tx_to tx
+  | _ => person_1
+  end.
+Definition congress_ifc : ContractInterface Congress.Msg :=
+match get_contract_interface chain4 congress_1 Congress.Msg with
+| Some x => x
+(* Using unpack_option here is extremely slow *)
+| None =>
+  @build_contract_interface
+    _ _
+    creator
+    (fun a m => deploy_congress)
+end.
+
+  (* person_1 adds person_1 and person_2 as members of congress *)
+Definition add_person p :=
+  congress_ifc.(send) 0 (Some (add_member p)).
+Definition chain5 : ChainBuilder :=
+  let acts := [build_act person_1 (add_person person_1);
+                build_act person_1 (add_person person_2)] in
+  unpack_result (add_block chain4 acts).
+Definition create_proposal_call :=
+  congress_ifc.(send) 0 (Some (create_proposal [cact_transfer person_3 3])).
+Definition chain6 : ChainBuilder :=
+  unpack_result (add_block chain5 [build_act person_1 create_proposal_call]).
+
+
 Definition chain_with_congress_deployed : LocalChain := lcb_lc chain6. (* chain6 is from LocalBlockchainTests.v *)
 Definition congress_chain := chain_with_congress_deployed.
 Definition congress_contract_base_addr := BoundedN.of_Z_const AddrSize 128%Z.
 
 Extract Constant defNumDiscards => "(4 * defNumTests)".
 
-Definition gCongressChainTraceList max_acts_per_block lc length := 
-  gLocalChainTraceList_fix lc (fun lc _ => 
+Definition gCongressChainTraceList max_acts_per_block lc length :=
+  gLocalChainTraceList_fix lc (fun lc _ =>
     gCongressActionNew lc 2) length max_acts_per_block.
 
-Definition forAllCongressTraces n := 
+Definition forAllCongressTraces n :=
   forAllTraces n congress_chain (gCongressChainTraceList 1).
-Notation "{{ P }} c {{ Q }}" := 
+Notation "{{ P }} c {{ Q }}" :=
   (pre_post_assertion 10 congress_chain (gCongressChainTraceList 1) c P Q)( at level 50).
 
 Open Scope string_scope.
-Definition debug_congress {A : Type} 
-                         `{Checkable A} 
-                          (lc : LocalChain) 
-                          (acts_opt : option (list Action)) 
-                          : A -> Checker := 
+Definition debug_congress {A : Type}
+                         `{Checkable A}
+                          (lc : LocalChain)
+                          (acts_opt : option (list Action))
+                          : A -> Checker :=
   whenFail (
     "LocalChain: " ++ show lc ++ nl ++
     "members: " ++ show (congressContractsMembers lc) ++ nl ++
@@ -52,13 +102,13 @@ Definition debug_congress {A : Type}
   ).
 Close Scope string_scope.
 
-Definition nr_cacts (msg : option Congress.Msg) := 
+Definition nr_cacts (msg : option Congress.Msg) :=
   match msg with
   | Some (create_proposal ls) => length ls
   | _ => 0
   end.
 
-(* What this says is that the number of actions to be performed by the congress never increases 
+(* What this says is that the number of actions to be performed by the congress never increases
    more than the actions that are added in proposals, ie. actions can't appear out of nowhere. *)
 (* If we replace '<=' with '<' QC finds a counterexample - a proposal can contain an empty list of actions, so they are equal before/after add_proposal *)
 Definition receive_state_well_behaved state msg new_state (resp_acts : list ActionBody) :=
@@ -68,36 +118,36 @@ Definition receive_state_well_behaved state msg new_state (resp_acts : list Acti
 Lemma a : forall state msg new_state resp_acts,
 Dec (receive_state_well_behaved state msg new_state resp_acts).
 Proof.
-  intros. unfold receive_state_well_behaved. 
-  constructor. 
+  intros. unfold receive_state_well_behaved.
+  constructor.
   apply le_dec.
 Qed.
 
-Instance receive_state_well_behaved_dec_ {state : Congress.State} 
-                                        {msg : option Congress.Msg} 
+Instance receive_state_well_behaved_dec_ {state : Congress.State}
+                                        {msg : option Congress.Msg}
                                         {new_state : Congress.State}
-                                        {resp_acts : list ActionBody} 
+                                        {resp_acts : list ActionBody}
                                         : Dec (receive_state_well_behaved state msg new_state resp_acts).
 Proof.
-  intros. 
-  unfold receive_state_well_behaved. 
-  constructor. 
+  intros.
+  unfold receive_state_well_behaved.
+  constructor.
   apply le_dec.
 Qed.
 
-(* Instance receive_state_well_behaved_checkable {state : Congress.State} 
-                                              {msg : option Congress.Msg} 
+(* Instance receive_state_well_behaved_checkable {state : Congress.State}
+                                              {msg : option Congress.Msg}
                                               {new_state : Congress.State}
-                                              {resp_acts : list ActionBody} 
-                                              : Checkable (receive_state_well_behaved_inner state msg new_state resp_acts). 
+                                              {resp_acts : list ActionBody}
+                                              : Checkable (receive_state_well_behaved_inner state msg new_state resp_acts).
 Proof. apply testDec. Qed. *)
 
 
 
-Definition receive_state_well_behaved_P (cctx : ContractCallContext) 
-                                        (old_state : Congress.State) 
-                                        (msg : Congress.Msg) 
-                                        (result : option (Congress.State * list ActionBody)) := 
+Definition receive_state_well_behaved_P (cctx : ContractCallContext)
+                                        (old_state : Congress.State)
+                                        (msg : Congress.Msg)
+                                        (result : option (Congress.State * list ActionBody)) :=
   match result with
   | Some (new_state, resp_acts) =>
     (receive_state_well_behaved old_state (Some msg) new_state resp_acts)?
@@ -117,14 +167,14 @@ Definition receive_state_well_behaved_P (cctx : ContractCallContext)
 
 (* A property about the way States are generated. *)
 (* It says that a State generated at some time slot cannot contain proposals later than this time slot. *)
-Definition state_proposals_proposed_in_valid_P (block_slot : nat) (state : Congress.State) := 
+Definition state_proposals_proposed_in_valid_P (block_slot : nat) (state : Congress.State) :=
   let proposals := map snd (FMap.elements (proposals state)) in
   forallb (fun p => proposed_in p <=? block_slot) proposals.
 
-Definition state_proposals_proposed_in_valid lc := 
+Definition state_proposals_proposed_in_valid lc :=
   let congress_state_map := lc_contract_state_deserialized Congress.State lc in
   checker match FMap.find congress_contract_base_addr congress_state_map with
-  | Some congress_state => 
+  | Some congress_state =>
     state_proposals_proposed_in_valid_P lc.(lc_slot) congress_state
   | None => false
   end.
@@ -138,8 +188,8 @@ Definition state_proposals_proposed_in_valid lc :=
 (* sanity check *)
 Definition add_block_actions_succeeds_P c_opt actions_opt :=
   isSomeCheck c_opt
-  (fun c => 
-    (debug_congress c actions_opt) 
+  (fun c =>
+    (debug_congress c actions_opt)
       (match actions_opt with
       | Some actions => (0 <? length actions) && isSome (my_add_block c actions)
       | None => false
@@ -149,14 +199,14 @@ Definition add_block_actions_succeeds_P c_opt actions_opt :=
 Instance shrinkAction : Shrink Action := {| shrink a := [a] |}.
 
 (* another sanity check *)
-Definition check_add_two_blocks_succeeds := 
-  (forAll3 
+Definition check_add_two_blocks_succeeds :=
+  (forAll3
     (optToVector 1 (gCongressActionNew chain_with_congress_deployed 2))
     (fun actions => returnGen (my_add_block chain_with_congress_deployed actions))
-    (fun _ c_opt => 
-      bindGenOpt (returnGen c_opt) 
+    (fun _ c_opt =>
+      bindGenOpt (returnGen c_opt)
       (fun c =>
-        acts <- (optToVector 1 (gCongressActionNew c 2)) ;; 
+        acts <- (optToVector 1 (gCongressActionNew c 2)) ;;
         returnGen (Some acts)))
     (fun _ c_opt actions_opt => add_block_actions_succeeds_P c_opt actions_opt)
   ).
@@ -165,7 +215,7 @@ Definition check_add_two_blocks_succeeds :=
 (* coqtop-stdout:+++ Passed 10000 tests (0 discards) *)
 
 
-Definition reachableFrom_congress (lc : LocalChain) pf : Checker := 
+Definition reachableFrom_congress (lc : LocalChain) pf : Checker :=
   @reachableFrom AddrSize lc (fun lc _ => gCongressChainTraceList 1 lc 2) pf.
 
 Notation "lc '~~>' pf" :=
@@ -177,7 +227,7 @@ Definition congress_has_votes_on_some_proposal lc :=
   match FMap.find congress_contract_base_addr congress_state_map with
   | Some state =>
     let proposals := map snd (FMap.elements (proposals state)) in
-    existsb (fun proposal => 
+    existsb (fun proposal =>
       0 <? FMap.size proposal.(votes)
     ) proposals
   | None => false
@@ -185,14 +235,14 @@ Definition congress_has_votes_on_some_proposal lc :=
 
 (* QuickChick (congress_chain ~~> congress_has_votes_on_some_proposal o next_lc_of_lcstep). *)
 (* coqtop-stdout:
-Begin Trace: 
+Begin Trace:
 step_action{
   Action{
-    act_from: 12%256, 
+    act_from: 12%256,
     act_body: (act_call 128%256, 0, vote_against_proposal 1)}};;
 step_action{
   Action{
-    act_from: 11%256, 
+    act_from: 11%256,
     act_body: (act_call 128%256, 5, create_proposal (call: 128%256, 4, create_proposal (call: 128%256, 4, vote_against_proposal 1)))}}
 End Trace
 Success - found witness satisfying the predicate!
@@ -203,30 +253,30 @@ Success - found witness satisfying the predicate!
 Definition congress_finished_a_vote (lc_step : @LocalChainStep AddrSize) :=
   match lc_step with
   | step_add_block _ _ _ => false
-  | step_action _ _ _ acts => 
-    let act_is_finish_vote (act : Action) := match act.(act_body) with 
-                                             | act_call _ _ msg => match deserialize Congress.Msg _ msg with 
-                                                                   | Some (Congress.finish_proposal _) => true 
-                                                                   | _ => false end  
+  | step_action _ _ _ acts =>
+    let act_is_finish_vote (act : Action) := match act.(act_body) with
+                                             | act_call _ _ msg => match deserialize Congress.Msg _ msg with
+                                                                   | Some (Congress.finish_proposal _) => true
+                                                                   | _ => false end
                                              | _ => false end in
     existsb act_is_finish_vote acts
   end.
 
 (* QuickChick (congress_chain ~~> congress_finished_a_vote). *)
-(* Begin Trace: 
+(* Begin Trace:
 step_action{
   Action{
-    act_from: 11%256, 
+    act_from: 11%256,
     act_body: (act_call 128%256, 3, finish_proposal 1)}};;
 step_action{
   Action{
-    act_from: 12%256, 
+    act_from: 12%256,
     act_body: (
       act_call 128%256, 0, create_proposal (
         call: 128%256, 0, create_proposal (
           call: 128%256, 2, change_rules Rules{
-            min_vote_count_permille: 450, 
-            margin_needed_permille: 467, 
+            min_vote_count_permille: 450,
+            margin_needed_permille: 467,
             debating_period_in_blocks: 2})))}}
 End Trace
 Success - found witness satisfying the predicate!
