execution/tests/CongressTests/Congress_BuggyTests.v
@@ -8,7 +8,6 @@ From ConCert Require Import Blockchain.
 From ConCert Require Import LocalBlockchain.
 From ConCert Require Import Serializable.
 From ConCert Require Import BoundedN.
-(* From ConCert Require Import LocalBlockchainTests. *)
 From ConCert Require Import Containers.
 From ConCert Require Import Congress_Buggy.
 Require Import ResultMonad.
@@ -37,7 +36,7 @@ Instance Builder : ChainBuilderType := LocalChainBuilderDepthFirst AddrSize.
 
 Let creator := BoundedN.of_Z_const AddrSize 10.
 
-Definition rules := {| 
+Definition rules := {|
   min_vote_count_permille := 200;
   margin_needed_permille := 501;
   debating_period_in_blocks := 0;
@@ -70,41 +69,41 @@ Definition exploit_example : option (Address * Builder) :=
           [add_creator] in
   do chain <- add_block chain act_bodies;
   Some (congress, chain).
-  
+
 Definition unpacked_exploit_example : Address * Builder :=
   unpack_option exploit_example.
 
-Definition gCongressChainTraceList max_acts_per_block lc length := 
-  gLocalChainTraceList_fix lc (fun lc _ => 
+Definition gCongressChainTraceList max_acts_per_block lc length :=
+  gLocalChainTraceList_fix lc (fun lc _ =>
   gCongressActionBuggy lc 2) length max_acts_per_block.
 
-Definition forAllCongressTraces n := 
+Definition forAllCongressTraces n :=
   forAllTraces n (lcb_lc (snd unpacked_exploit_example)) (gCongressChainTraceList 1).
-Notation "{{ P }} c {{ Q }}" := 
+Notation "{{ P }} c {{ Q }}" :=
   (pre_post_assertion 2 (lcb_lc (snd unpacked_exploit_example)) (gCongressChainTraceList 1) c P Q)( at level 50).
 Local Close Scope Z_scope.
 
 Definition num_cacts_in_state state :=
   sumnat (fun '(k, v) => length (actions v)) (FMap.elements (proposals state)).
 
-Definition num_cacts_safe_P (msg : Congress_Buggy.Msg) 
+Definition num_cacts_safe_P (msg : Congress_Buggy.Msg)
                             (resp_acts : list ActionBody)
-                            (old_state : Congress_Buggy.State) 
+                            (old_state : Congress_Buggy.State)
                             (new_state : Congress_Buggy.State) :=
   let nr_cacts := match msg with
                   | create_proposal ls => length ls
                   | _ => 0
-                  end in 
+                  end in
   num_cacts_in_state new_state + length resp_acts <=?
   num_cacts_in_state old_state + nr_cacts.
 
-Definition receive_state_well_behaved_P (cctx : ContractCallContext) 
-                                        (old_state : Congress_Buggy.State) 
-                                        (msg : Congress_Buggy.Msg) 
-                                        (result : option (Congress_Buggy.State * list ActionBody)) := 
+Definition receive_state_well_behaved_P (cctx : ContractCallContext)
+                                        (old_state : Congress_Buggy.State)
+                                        (msg : Congress_Buggy.Msg)
+                                        (result : option (Congress_Buggy.State * list ActionBody)) :=
   match result with
   | Some (new_state, resp_acts) =>
-    checker (num_cacts_safe_P msg resp_acts old_state new_state) 
+    checker (num_cacts_safe_P msg resp_acts old_state new_state)
   | _ => checker false
   end.
 
@@ -115,13 +114,13 @@ Definition receive_state_well_behaved_P (cctx : ContractCallContext)
 ). *)
 
 (* coqtop-stdout:
-Begin Trace: 
+Begin Trace:
 step_action{
   Action{
-    act_from: 10%256, 
+    act_from: 10%256,
     act_body: (act_call 128%256, 0, create_proposal (transfer: 10%256, 1))}};;
 step_action{
-  Action{act_from: 10%256, 
+  Action{act_from: 10%256,
   act_body: (act_call 128%256, 0, finish_proposal 1)}}
 End Trace
 
