execution/tests/FA2Tests/FA2TokenTests.v
@@ -1,7 +1,5 @@
 From ConCert Require Import Blockchain LocalBlockchain FA2Token FA2Interface.
 From ConCert Require Import Serializable.
-From ConCert Require Import LocalBlockchainTests.
-(* From Coq Require Import Morphisms. *)
 From ConCert Require Import Extras.
 From ConCert Require Import Containers.
 From ConCert Require Import BoundedN.
@@ -10,7 +8,7 @@ Require Import ZArith Strings.String.
 
 From QuickChick Require Import QuickChick. Import QcNotation.
 From ExtLib.Structures Require Import Functor Applicative.
-From ConCert.Execution.QCTests Require Import 
+From ConCert.Execution.QCTests Require Import
 	TestUtils ChainPrinters SerializablePrinters TraceGens FA2Printers TestContracts.
 From RecordUpdate Require Import RecordUpdate.
 From Coq Require Import List.
@@ -71,7 +69,7 @@ Definition token_metadata_0 : token_metadata := {|
 
 Definition token_setup (hook_addr : option Address): FA2Token.Setup := {|
   setup_total_supply := [];
-  setup_tokens := FMap.add 0%N token_metadata_0 FMap.empty; 
+  setup_tokens := FMap.add 0%N token_metadata_0 FMap.empty;
   initial_permission_policy := policy_all;
   transfer_hook_addr_ := hook_addr;
 
@@ -80,24 +78,24 @@ Definition token_setup (hook_addr : option Address): FA2Token.Setup := {|
 Definition token_contract_base_addr : Address := BoundedN.of_Z_const AddrSize 128%Z.
 Definition fa2hook_setup : HookSetup := {|
   hook_fa2_caddr_ := token_contract_base_addr;
-  hook_policy_ := policy_self_only; 
+  hook_policy_ := policy_self_only;
 |}.
 Definition deploy_fa2hook := create_deployment 0 hook_contract fa2hook_setup.
 Definition fa2hook_contract_addr : Address := BoundedN.of_Z_const AddrSize 130%Z.
 
-Definition deploy_fa2token_with_transfer_hook : @ActionBody Base := 
+Definition deploy_fa2token_with_transfer_hook : @ActionBody LocalChainBase :=
   create_deployment 0 FA2Token.contract (token_setup (Some fa2hook_contract_addr)) .
-Definition deploy_fa2token_without_transfer_hook : @ActionBody Base := 
+Definition deploy_fa2token_without_transfer_hook : @ActionBody LocalChainBase :=
   create_deployment 0 FA2Token.contract (token_setup None).
 
 Definition token_client_setup := build_clientsetup token_contract_base_addr.
-Definition deploy_fa2token_client : @ActionBody Base := create_deployment 0 client_contract token_client_setup.
+Definition deploy_fa2token_client : @ActionBody LocalChainBase := create_deployment 0 client_contract token_client_setup.
 Definition client_contract_addr : Address := BoundedN.of_Z_const AddrSize 129%Z.
 
 
 
-Definition chain_with_token_deployed_with_hook : LocalChain :=  
-  unpack_option (my_add_block lc_initial 
+Definition chain_with_token_deployed_with_hook : LocalChain :=
+  unpack_option (my_add_block lc_initial
   [
     build_act creator (act_transfer person_1 10);
     build_act creator (act_transfer person_2 10);
@@ -107,8 +105,8 @@ Definition chain_with_token_deployed_with_hook : LocalChain :=
     build_act creator deploy_fa2hook
   ]).
 
-Definition chain_with_token_deployed_without_hook : LocalChain :=  
-  unpack_option (my_add_block lc_initial 
+Definition chain_with_token_deployed_without_hook : LocalChain :=
+  unpack_option (my_add_block lc_initial
   [
     build_act creator (act_transfer person_1 10);
     build_act creator (act_transfer person_2 10);
@@ -120,32 +118,32 @@ Definition chain_with_token_deployed_without_hook : LocalChain :=
 Definition client_other_msg := @other_msg _ FA2ClientMsg _.
 
 Definition call_client_is_op_act :=
-  let params := Build_is_operator_param 
+  let params := Build_is_operator_param
       (Build_operator_param zero_address zero_address all_tokens)
-      (Build_callback is_operator_response None) in 
+      (Build_callback is_operator_response None) in
   let msg := client_other_msg (Call_fa2_is_operator params) in
   act_call client_contract_addr 0%Z (serialize ClientMsg _ msg).
 
 Definition chain_with_transfer_hook :=
-  unpack_option (my_add_block chain_with_token_deployed_with_hook 
+  unpack_option (my_add_block chain_with_token_deployed_with_hook
   [
     build_act person_1 (act_call token_contract_base_addr 10%Z (serialize _ _ (msg_create_tokens 0%N))) ;
     build_act person_2 (act_call token_contract_base_addr 10%Z (serialize _ _ (msg_create_tokens 0%N)))
   ]).
 
 Definition chain_without_transfer_hook :=
-  unpack_option (my_add_block chain_with_token_deployed_without_hook 
+  unpack_option (my_add_block chain_with_token_deployed_without_hook
   [
     build_act person_1 (act_call token_contract_base_addr 10%Z (serialize _ _ (msg_create_tokens 0%N))) ;
     build_act person_2 (act_call token_contract_base_addr 10%Z (serialize _ _ (msg_create_tokens 0%N)))
   ]).
 
-Definition client_state lc := 
+Definition client_state lc :=
   match (FMap.find client_contract_addr lc.(lc_contract_state)) with
   | Some state => deserialize ClientState _ state
   | None => None
   end.
-Definition token_state lc := 
+Definition token_state lc :=
   match (FMap.find token_contract_base_addr lc.(lc_contract_state)) with
   | Some state => deserialize FA2Token.State _ state
   | None => None
@@ -163,9 +161,9 @@ Module MG := FA2Gens.FA2Gens TestInfo. Import MG.
 
 Definition chain_with_transfer_hook_token_state : FA2Token.State := unpack_option (token_state chain_with_transfer_hook).
 (* Compute (show chain_with_transfer_hook_token_state). *)
-Definition gFA2TokenActionChainTraceList max_acts_per_block lc length := 
+Definition gFA2TokenActionChainTraceList max_acts_per_block lc length :=
   gLocalChainTraceList_fix lc (fun lc _ => gFA2TokenAction lc) length max_acts_per_block.
-Definition gFA2ClientChainTraceList max_acts_per_block lc length := 
+Definition gFA2ClientChainTraceList max_acts_per_block lc length :=
   gLocalChainTraceList_fix lc (fun lc _ => gClientAction lc) length max_acts_per_block.
 
 (* Sample (gFA2TokenAction chain_with_transfer_hook). *)
@@ -177,18 +175,18 @@ Notation "{{ P }} c {{ Q }} chain" := (pre_post_assertion 7 chain (gFA2ChainTrac
 Extract Constant defNumDiscards => "(10 * defNumTests)".
 
 Local Open Scope Z_scope.
-Definition transfer_state_update_correct prev_state next_state transfers := 
+Definition transfer_state_update_correct prev_state next_state transfers :=
   let balance_diffs_map : FMap (Address * token_id) Z := fold_left (fun current_diff_map trx =>
     (* subtract amount from sender *)
-    let m1 := 
+    let m1 :=
       let amount := Z.of_N (trx.(amount)) in
       let from_key := (trx.(from_), trx.(transfer_token_id)) in
       match FMap.find from_key current_diff_map with
       | Some current_diff => FMap.add from_key (current_diff - amount) current_diff_map
-      | None => FMap.add from_key (-amount) current_diff_map 
+      | None => FMap.add from_key (-amount) current_diff_map
       end in
     (* add amount to receiver *)
-    let m2 := 
+    let m2 :=
       let amount := Z.of_N (trx.(amount)) in
       let to_key := (trx.(to_), trx.(transfer_token_id)) in
       match FMap.find to_key m1 with
@@ -204,7 +202,7 @@ Definition transfer_state_update_correct prev_state next_state transfers :=
     let balance_after := Z.of_N (address_balance tokenid addr next_state) in
     (* check that balance_diff is equal to the difference in recorded balance *)
     (balance_before + balance_diff) =? balance_after in
-  forEachMapEntry balance_diffs_map balance_update_correct. 
+  forEachMapEntry balance_diffs_map balance_update_correct.
 Local Close Scope Z_scope.
 
 Definition msg_is_transfer (cstate : FA2Token.State) (msg : FA2Token.Msg) :=
@@ -215,8 +213,8 @@ Definition msg_is_transfer (cstate : FA2Token.State) (msg : FA2Token.Msg) :=
 
 Definition post_transfer_correct (cctx : ContractCallContext) old_state msg (result_opt : option (FA2Token.State * list ActionBody)) :=
   match result_opt with
-  | Some (new_state, _) => 
-    let transfers := 
+  | Some (new_state, _) =>
+    let transfers :=
       match msg with
       | msg_transfer transfers => transfers
       | _ => []
@@ -226,32 +224,32 @@ Definition post_transfer_correct (cctx : ContractCallContext) old_state msg (res
   end.
 
 (* QuickChick (
-  {{ msg_is_transfer }} 
-    FA2Token.contract 
+  {{ msg_is_transfer }}
+    FA2Token.contract
   {{ post_transfer_correct }}
   chain_without_transfer_hook). *)
 (* 14 seconds, max size 7, 1 act per block *)
 (* coqtop-stdout:+++ Passed 10000 tests (12283 discards) *)
 
-Definition transfer_balances_correct (step : @LocalChainStep AddrSize) := 
+Definition transfer_balances_correct (step : @LocalChainStep AddrSize) :=
   match step with
   | step_add_block _ _ _ => false ==> true
   | step_action prev_lc _ next_lc [act] =>
     match act.(act_body) with
     | act_call _ _ msg =>
       match deserialize FA2Token.Msg _ msg with
-      | Some (msg_transfer transfers) => 
+      | Some (msg_transfer transfers) =>
         (* check that next_lc is updated correctly from prev_lc according to the transfers *)
         let prev_state := token_state prev_lc in
         let next_state := token_state next_lc in
         match (prev_state, next_state) with
-        | (Some prev_state, Some next_state) => 
+        | (Some prev_state, Some next_state) =>
           whenFail (show prev_state ++ nl ++ show next_state)
           (checker (transfer_state_update_correct prev_state next_state transfers))
         | _ => false ==> true
         end
       | _ => false ==> true
-      end 
+      end
     | _ => false ==> true
     end
   | _ => false ==> true
@@ -260,15 +258,15 @@ Definition transfer_balances_correct (step : @LocalChainStep AddrSize) :=
 (* QuickChick (forAllFA2Traces chain_with_transfer_hook 1 transfer_balances_correct). *)
 
 
-Definition transfer_satisfies_policy sender trx state : Checker := 
+Definition transfer_satisfies_policy sender trx state : Checker :=
   (* check if sender is an operator, and permission to transfer the specified token_id *)
   let policy := state.(permission_policy) in
-  let is_valid_operator_transfer : Checker := 
+  let is_valid_operator_transfer : Checker :=
     match FMap.find trx.(from_) state.(operators) with
-    | Some ops_map => 
+    | Some ops_map =>
       match FMap.find sender ops_map with
       | Some all_tokens => checker true
-      | Some (some_tokens token_ids) => 
+      | Some (some_tokens token_ids) =>
         whenFail "operator didn't have sufficient token_id permissions"
         (checker (existsb (N.eqb trx.(transfer_token_id)) token_ids))
       | None => checker false
@@ -281,7 +279,7 @@ Definition transfer_satisfies_policy sender trx state : Checker :=
     (* no transfers allowed *)
     | (self_transfer_denied, operator_transfer_denied) => checker false
     (* only self transfer allowed - check sender is equal to 'from' *)
-    | (self_transfer_permitted, operator_transfer_denied) => 
+    | (self_transfer_permitted, operator_transfer_denied) =>
       whenFail "operator transfer was denied, but sender != from"
       (address_eqb sender trx.(from_))
     | (self_transfer_denied, operator_transfer_permitted) =>
@@ -289,19 +287,19 @@ Definition transfer_satisfies_policy sender trx state : Checker :=
       then whenFail "self transfer was denied but got transfer with sender = from" false
       else is_valid_operator_transfer
     | (self_transfer_permitted, operator_transfer_permitted) =>
-    if address_eqb sender trx.(from_) 
+    if address_eqb sender trx.(from_)
     then checker true
-    else is_valid_operator_transfer 
+    else is_valid_operator_transfer
   end.
 
-Definition get_transfers (acts : list Action) : list (Address * list FA2Interface.transfer) := 
-  fold_left (fun trxs act => 
+Definition get_transfers (acts : list Action) : list (Address * list FA2Interface.transfer) :=
+  fold_left (fun trxs act =>
     match act.(act_body) with
     | act_call _ _ msg =>
       match deserialize FA2Token.Msg _ msg with
       | Some (msg_transfer transfers) => (act.(act_from), transfers) :: trxs
       | _ => trxs
-      end 
+      end
     | _ => trxs
     end) acts [].
 
@@ -313,16 +311,16 @@ Definition transfer_satisfies_policy_P (step : @LocalChainStep AddrSize) : Check
   | Some state =>
       conjoin_map (fun sender_trxs_pair =>
         conjoin_map (fun trx =>
-          transfer_satisfies_policy (fst sender_trxs_pair) trx state 
+          transfer_satisfies_policy (fst sender_trxs_pair) trx state
           ) (snd sender_trxs_pair)
       ) transfers
   | None => checker false
   end.
 
-Definition showStateWhenFail (step : @LocalChainStep AddrSize) := 
+Definition showStateWhenFail (step : @LocalChainStep AddrSize) :=
   let prev_lc := prev_lc_of_lcstep step in
   let next_lc := next_lc_of_lcstep step in
-  whenFail 
+  whenFail
   ("Failed on step: " ++ nl ++ show step ++ nl ++
   match (token_state prev_lc, token_state next_lc) with
   | (Some prev_state, Some next_state) =>
@@ -333,7 +331,7 @@ Definition showStateWhenFail (step : @LocalChainStep AddrSize) :=
   | _ => ""
   end).
 
-(* QuickChick (forAllFA2Traces 7 transfer_satisfies_policy_P). *)
+(* QuickChick (forAllFA2Traces chain_with_transfer_hook 7 transfer_satisfies_policy_P). *)
 (* coqtop-stdout:+++ Passed 10000 tests (2432 discards) *)
 
 
@@ -350,11 +348,11 @@ Definition single_update_op_correct (new_state : FA2Token.State) (op : update_op
   end.
 
 
-(* This property asserts that if an update_operator action contains multiple updates for the same operator, 
+(* This property asserts that if an update_operator action contains multiple updates for the same operator,
    the LAST operation in the list must take effect *)
-Definition last_update_operator_occurrence_takes_effect (update_ops : list update_operator) 
+Definition last_update_operator_occurrence_takes_effect (update_ops : list update_operator)
                                                         (new_state : FA2Token.State) :=
-  let last_ops : FMap (Address * Address) update_operator := 
+  let last_ops : FMap (Address * Address) update_operator :=
     fold_left (fun acc update_op =>
     let param := match update_op with
       | add_operator param => param
@@ -374,13 +372,13 @@ Definition msg_is_update_operator (cstate : FA2Token.State) (msg : FA2Token.Msg)
   | _ => false
   end.
 
-Definition post_last_update_operator_occurrence_takes_effect (cctx : ContractCallContext) 
-                                 (old_state : FA2Token.State) 
-                                 msg 
+Definition post_last_update_operator_occurrence_takes_effect (cctx : ContractCallContext)
+                                 (old_state : FA2Token.State)
+                                 msg
                                  (result_opt : option (FA2Token.State * list ActionBody)) :=
   match result_opt with
-  | Some (new_state, _) => 
-    let update_ops := 
+  | Some (new_state, _) =>
+    let update_ops :=
       match msg with
       | msg_update_operators ops => ops
       | _ => []
@@ -405,24 +403,24 @@ Definition post_last_update_operator_occurrence_takes_effect (cctx : ContractCal
   match act_opt with
   | Some act =>
     match (my_add_block chain_with_token_deployed [act]) with
-    | Some c => gFA2TokenAction c 
+    | Some c => gFA2TokenAction c
     | None => returnGen None
     end
   | None => returnGen None
   end)
-  (fun act1_opt act2_opt => 
+  (fun act1_opt act2_opt =>
     match (act1_opt, act2_opt) with
-    | (Some act1, Some act2) => 
-      whenFail 
+    | (Some act1, Some act2) =>
+      whenFail
         ("execution failed:" ++ nl
-        ++ show (my_add_block chain_with_token_deployed [act1])) 
+        ++ show (my_add_block chain_with_token_deployed [act1]))
         (
-          let c_opt := my_add_block chain_with_token_deployed [act1] in 
+          let c_opt := my_add_block chain_with_token_deployed [act1] in
           match c_opt with
           | Some c => checker (isSome (my_add_block c [act2]))
           | None => whenFail "empty chain" false
           end
         )
     | _ => whenFail "empty act" false
-    end) 
+    end)
 ). *)
