execution/tests/TestUtils.v
@@ -13,11 +13,32 @@ From ConCert Require Import BoundedN ChainedList. Import BoundedN.Stdpp.
 From Coq Require Import List. Import ListNotations.
 From Coq Require Import Program.Basics.
 Require Import Containers.
+Require Import ResultMonad.
 
 Global Definition AddrSize := (2^8)%N.
 
-Instance LocalChainBase : ChainBase := LocalChainBase AddrSize.
-Instance LocalChainBuilder : ChainBuilderType := LocalChainBuilderDepthFirst AddrSize.
+Global Instance LocalChainBase : ChainBase := LocalChainBase AddrSize.
+(* Global Instance LocalChainBuilder : ChainBuilderType := LocalChainBuilderDepthFirst AddrSize. *)
+Global Instance ChainBuilder : ChainBuilderType := LocalChainBuilderDepthFirst AddrSize.
+
+Definition creator : Address :=
+  BoundedN.of_Z_const AddrSize 10.
+Definition person_1 : Address :=
+  BoundedN.of_Z_const AddrSize 11.
+Definition person_2 : Address :=
+  BoundedN.of_Z_const AddrSize 12.
+Definition person_3 : Address :=
+  BoundedN.of_Z_const AddrSize 13.
+
+Definition unpack_result {T E} (r : result T E) :=
+  match r return match r with
+                  | Ok _ => T
+                  | Err _ => E
+                  end with
+  | Ok t => t
+  | Err e => e
+  end.
+
 
 Notation "f 'o' g" := (compose f g) (at level 50).
 
@@ -33,23 +54,23 @@ Definition isSome {A : Type} (a : option A) := negb (isNone a).
 Fixpoint mkMapFromLists {A B : Type}
                        (a_eqb : A -> A -> bool)
                        (default : B)
-                       (l : list A) 
+                       (l : list A)
                        (lb : list B)
                        : A -> B :=
   match (l,lb) with
   | ([],[]) => fun x => default
-  | (a::l', b::lb') => 
-    fun (x : A) => if a_eqb x a then b else (mkMapFromLists a_eqb default l' lb') x 
+  | (a::l', b::lb') =>
+    fun (x : A) => if a_eqb x a then b else (mkMapFromLists a_eqb default l' lb') x
   | (_,_) => fun x => default
   end.
 Definition string_of_FMap {A B : Type}
                          `{countable.Countable A}
                          `{base.EqDecision A}
-                          (showA : A -> string) 
-                          (showB : B -> string) 
+                          (showA : A -> string)
+                          (showB : B -> string)
                           (m : FMap A B) : string :=
   "[" ++
-    String.concat "; " (map (fun p => showA (fst p) ++ "-->" ++ showB (snd p)) (FMap.elements m))
+    String.concat "; " (map (fun '(a, b) => showA a ++ "-->" ++ showB b) (FMap.elements m))
   ++ "]".
 
 Definition filter_FMap {A B : Type}
@@ -57,7 +78,7 @@ Definition filter_FMap {A B : Type}
                       `{base.EqDecision A}
                        (f : (A * B) -> bool)
                        (m : FMap A B)
-                       : FMap A B := 
+                       : FMap A B :=
   let l := FMap.elements m in
   let filtered_l := List.filter (fun p => f p) l in
   FMap.of_list filtered_l.
@@ -67,7 +88,7 @@ Definition map_values_FMap {A B C: Type}
                       `{base.EqDecision A}
                        (f : B -> C)
                        (m : FMap A B)
-                       : FMap A C := 
+                       : FMap A C :=
   let l := FMap.elements m in
   let mapped_l := List.map (fun p => (fst p, f (snd p))) l in
   FMap.of_list mapped_l.
@@ -77,7 +98,7 @@ Definition map_filter_FMap {A B C: Type}
                       `{base.EqDecision A}
                        (f : (A * B) -> option C)
                        (m : FMap A B)
-                       : FMap A C := 
+                       : FMap A C :=
   let l := FMap.elements m in
   let mapped_l := List.fold_left (fun acc p => match f p with
                                                | Some c => ((fst p), c) :: acc
@@ -85,15 +106,15 @@ Definition map_filter_FMap {A B C: Type}
                                                end  ) l [] in
   FMap.of_list mapped_l.
 
-Definition FMap_find_ {A B : Type}                           
+Definition FMap_find_ {A B : Type}
 										`{countable.Countable A}
 										`{base.EqDecision A}
 										 (k : A)
 										 (m : FMap A B)
-										 (default : B)  := 
-	match FMap.find k m with 
-	| Some v => v 
-	| None => default 
+										 (default : B)  :=
+	match FMap.find k m with
+	| Some v => v
+	| None => default
 	end.
 
 (* Utils for Show instances *)
@@ -102,10 +123,10 @@ Definition empty_str : string := "".
 Definition sep : string := ", ".
 Derive Show for unit.
 
-Definition deserialize_to_string {ty : Type} 
+Definition deserialize_to_string {ty : Type}
                                 `{Serializable ty}
-                                `{Show ty} 
-                                 (s : SerializedValue) : string := 
+                                `{Show ty}
+                                 (s : SerializedValue) : string :=
   match @deserialize ty _ s with
   | Some v => show v
   | None => "?"
@@ -114,7 +135,7 @@ Definition deserialize_to_string {ty : Type}
 Instance showFMap {A B : Type}
                  `{countable.Countable A}
                  `{base.EqDecision A}
-                 `{Show A} 
+                 `{Show A}
                  `{Show B}
                   : Show (FMap A B) :=
 {|
@@ -129,15 +150,15 @@ Definition lc_account_balance lc addr : option Amount := (FMap.find addr (@lc_ac
 
 Definition lc_contract_state_deserialized (state : Type) `{Serializable state} lc : FMap Address state :=
   let els_list : list (Address * SerializedValue) := FMap.elements (lc_contract_state lc) in
-  FMap.of_list (List.fold_left 
-                (fun acc p => 
+  FMap.of_list (List.fold_left
+                (fun acc p =>
                   match @deserialize state _ (snd p) with
                   | Some state => (fst p, state) :: acc
                   | None => acc
-                  end)  
+                  end)
                 els_list []).
 
-Definition lc_contract_owners : LocalChain -> FMap Address Address := 
+Definition lc_contract_owners : LocalChain -> FMap Address Address :=
   (map_values_FMap owner) o (lc_contract_state_deserialized Congress.State).
 
 Open Scope bool_scope.
@@ -145,16 +166,16 @@ Open Scope bool_scope.
 Definition lc_proposals (lc : LocalChain) : FMap Address (FMap ProposalId Proposal) :=
   map_values_FMap proposals (lc_contract_state_deserialized Congress.State lc).
 
-  
-Definition lc_contract_members_and_proposals_new_voters (lc : LocalChain) : FMap Address (FMap Address (list ProposalId)) := 
-  map_filter_FMap (fun p => 
+
+Definition lc_contract_members_and_proposals_new_voters (lc : LocalChain) : FMap Address (FMap Address (list ProposalId)) :=
+  map_filter_FMap (fun p =>
     let contract_addr := fst p in
     let state := snd p in
     let candidate_members := (map fst o FMap.elements) (members state) in
     let proposals_pairs := FMap.elements (proposals state) in
     if (0 <? length candidate_members) && (0 <? length proposals_pairs)
-    then 
-      let voters_to_proposals : FMap Address (list ProposalId) := 
+    then
+      let voters_to_proposals : FMap Address (list ProposalId) :=
         List.fold_left (fun acc m =>
         let unvoted_proposals : list (ProposalId * Proposal) := List.filter (fun p => match FMap.find m (votes (snd p)) with
                                                   | Some _ => false
@@ -167,12 +188,12 @@ Definition lc_contract_members_and_proposals_new_voters (lc : LocalChain) : FMap
       ) candidate_members FMap.empty in
       Some voters_to_proposals
     else None
-  ) (lc_contract_state_deserialized Congress.State lc) 
+  ) (lc_contract_state_deserialized Congress.State lc)
 .
 
-Definition lc_contract_members_and_proposals_with_votes (lc : LocalChain) 
-                                                        : FMap Address (FMap Address (list ProposalId)) := 
-  map_filter_FMap (fun p => 
+Definition lc_contract_members_and_proposals_with_votes (lc : LocalChain)
+                                                        : FMap Address (FMap Address (list ProposalId)) :=
+  map_filter_FMap (fun p =>
     let contract_addr := fst p in
     let state := snd p in
     let members : list Address := (map fst o FMap.elements) (members state) in
@@ -183,7 +204,7 @@ Definition lc_contract_members_and_proposals_with_votes (lc : LocalChain)
       fold_left (fun acc m => FMap.add m propIds acc) members FMap.empty
     )
     else None
-  ) (lc_contract_state_deserialized Congress.State lc) 
+  ) (lc_contract_state_deserialized Congress.State lc)
 .
 
 (* Utils for Generators *)
@@ -192,14 +213,14 @@ Definition elems_opt {A : Type} (l : list A) : G (option A) :=
   match l with
   | x::xs => liftM Some (elems_ x xs)
   | _ => returnGen None end.
-  
+
 Definition returnGenSome {A : Type} (a : A) := returnGen (Some a).
 
 
-Definition sampleFMapOpt {A B : Type}                           
+Definition sampleFMapOpt {A B : Type}
                         `{countable.Countable A}
                         `{base.EqDecision A}
-                         (m : FMap A B) 
+                         (m : FMap A B)
                          : G (option (A * B)) :=
   let els := FMap.elements m in
   match els with
@@ -207,11 +228,11 @@ Definition sampleFMapOpt {A B : Type}
   | [] => returnGen None
   end.
 
-Definition sampleFMapOpt_filter {A B : Type}                           
+Definition sampleFMapOpt_filter {A B : Type}
                         `{countable.Countable A}
                         `{base.EqDecision A}
                          (m : FMap A B)
-                         (f : (A * B) -> bool) 
+                         (f : (A * B) -> bool)
                          : G (option (A * B)) :=
   let els := FMap.elements m in
   match els with
@@ -220,10 +241,10 @@ Definition sampleFMapOpt_filter {A B : Type}
   end.
 
 Definition sample2UniqueFMapOpt
-												 {A B : Type}                           
+												 {A B : Type}
                         `{countable.Countable A}
                         `{base.EqDecision A}
-                         (m : FMap A B) 
+                         (m : FMap A B)
 												 : G (option ((A * B) * (A * B))) :=
 	bindGenOpt (sampleFMapOpt m) (fun p1 =>
 		let key1 := fst p1 in
@@ -241,9 +262,9 @@ Definition gAccountAddrFromLocalChain lc : G (option Address) :=
   returnGen match p with
   | Some (addr, _) => Some addr
   | None => None
-  end. 
+  end.
 
-Fixpoint remove_multipe_FMap {A B : Type}                           
+Fixpoint remove_multipe_FMap {A B : Type}
                             `{countable.Countable A}
                             `{base.EqDecision A}
                              (m : FMap A B)
@@ -260,7 +281,7 @@ Definition gAddrFromLCWithoutAddrs lc addrs : G (option Address) :=
   returnGen match p with
   | Some (addr, _) => Some addr
   | None => None
-  end. 
+  end.
 
 Definition gAccountAddrFromLCWithoutAddrs lc addrs : G (option Address) :=
   let acc_bals_sub := remove_multipe_FMap (@lc_account_balances AddrSize lc) addrs in
@@ -268,14 +289,14 @@ Definition gAccountAddrFromLCWithoutAddrs lc addrs : G (option Address) :=
   returnGen match p with
   | Some (addr, _) => Some addr
   | None => None
-  end. 
+  end.
 
 Definition gContractAddrFromLocalChain lc : G (option Address) :=
   p <- sampleFMapOpt (@lc_contracts AddrSize lc) ;;
   returnGen match p with
   | Some (addr, _) => Some addr
   | None => None
-  end. 
+  end.
 
 Definition gContractAddrFromLCWithoutAddrs lc addrs : G (option Address) :=
   let contracts_sub := remove_multipe_FMap (@lc_contracts AddrSize lc) addrs in
@@ -283,7 +304,7 @@ Definition gContractAddrFromLCWithoutAddrs lc addrs : G (option Address) :=
   returnGen match p with
   | Some (addr, _) => Some addr
   | None => None
-  end. 
+  end.
 
 Definition gAccountBalanceFromLocalChain lc : G (option (Address * Amount)) :=
   sampleFMapOpt (@lc_account_balances AddrSize lc).
@@ -303,12 +324,12 @@ Definition gContractSateFromLCWithoutAddrs lc addrs : G (option (Address * Seria
 Definition gZPositive := liftM Z.of_nat arbitrary.
 Definition gZPositiveSized n := liftM Z.of_nat (arbitrarySized n).
 
-(* Although the type is G (option ...) it will never generate None values. 
+(* Although the type is G (option ...) it will never generate None values.
    Perhaps this is where we should use generators with property proof relevance? Future work... *)
 	 Definition gBoundedNOpt (bound : N): G (option (BoundedN.BoundedN bound)) :=
 	 n <- arbitrarySized (N.to_nat bound) ;; (* we exploit that arbitrarySized n on nats automatically bounds the value by <= n *)
 	 returnGen (@decode_bounded bound (Pos.of_nat n)).
- 
+
  Definition gBoundedN : G (BoundedN.BoundedN AddrSize) :=
 	 bn <- gBoundedNOpt AddrSize ;;
 	 returnGen match bn with
@@ -316,7 +337,7 @@ Definition gZPositiveSized n := liftM Z.of_nat (arbitrarySized n).
 		 (** The None case should never happen since 'arbitrarySized' on AddrSize already ensures that
 				 n <= AddrSized. **)
 		 | None => BoundedN.of_Z_const AddrSize 0
-	 end. 
+	 end.
 
 Instance genBoundedN : Gen (BoundedN.BoundedN AddrSize) :=
   {|
@@ -326,14 +347,14 @@ Instance genBoundedN : Gen (BoundedN.BoundedN AddrSize) :=
 Instance genAddress : Gen (@Address LocalChainBase) :=
   {|
     (* I could have just written 'arbitrary' here, but this is more explicit; and i like explicit code *)
-    arbitrary := @arbitrary (BoundedN.BoundedN AddrSize) genBoundedN 
+    arbitrary := @arbitrary (BoundedN.BoundedN AddrSize) genBoundedN
   |}.
 
 Definition gDeploymentAction {Setup Msg State : Type}
                             `{Serializable Setup}
                             `{Serializable Msg}
                             `{Serializable State}
-                             {BaseTypes : ChainBase} 
+                             {BaseTypes : ChainBase}
                              (contract : @Contract BaseTypes Setup Msg State _ _ _)
                              (setup : Setup) : G ActionBody :=
   amount <- arbitrary ;;
@@ -342,8 +363,8 @@ Definition gDeploymentAction {Setup Msg State : Type}
 
 (* Helper generator and show instance for arbitrary FMaps *)
 
-Fixpoint gFMapSized {A B : Type} 
-                    {gA : G A} 
+Fixpoint gFMapSized {A B : Type}
+                    {gA : G A}
                     {gB : G B}
                     `{countable.Countable A}
                     `{base.EqDecision A}
@@ -354,12 +375,12 @@ Fixpoint gFMapSized {A B : Type}
     a <- gA ;;
     b <- gB ;;
     m <- @gFMapSized _ _ gA gB _ _ _ n' ;;
-    returnGen (FMap.add a b m)  
+    returnGen (FMap.add a b m)
   end.
 
 Fixpoint gFMapFromInput {A B : Type}
                        `{countable.Countable A}
-                       `{base.EqDecision A}     
+                       `{base.EqDecision A}
                         (l1 : list A)
                         (l2 : list B)
                         : G (FMap A B) :=
@@ -368,8 +389,8 @@ Fixpoint gFMapFromInput {A B : Type}
   | (_, _) => returnGen FMap.empty
   end.
 
-Instance genFMapSized {A B : Type} 
-                     `{Gen A} 
+Instance genFMapSized {A B : Type}
+                     `{Gen A}
                      `{Gen B}
                      `{countable.Countable A}
                      `{base.EqDecision A}
@@ -381,12 +402,12 @@ Instance genFMapSized {A B : Type}
 (* Sample (@gFMapSized nat nat arbitrary arbitrary _ _ _ 1). *)
 
 Fixpoint vectorOfCount {A : Type}
-                      `{countable.Countable A} 
+                      `{countable.Countable A}
                        (default : A)
-                       (n : nat) : G (list A) := 
+                       (n : nat) : G (list A) :=
   match n with
   | 0    => returnGen []
-  | S n' => 
+  | S n' =>
     match (countable.decode o Pos.of_nat) n with
     | Some a => liftM (cons a) (vectorOfCount default n')
     | None => liftM (cons default) (vectorOfCount default n')
@@ -411,12 +432,12 @@ Fixpoint shrinkListTo {A : Type} maxSize (l : list A) : list A:=
             end
   end.
 
-Fixpoint gInterp_type (t : SerializedType) : G (interp_type t) := 
+Fixpoint gInterp_type (t : SerializedType) : G (interp_type t) :=
   match t with
   | ser_unit => returnGen tt
   | ser_int => @arbitrary Z _
   | ser_bool => arbitrary
-  | ser_pair a b => liftM2 pair (gInterp_type a) (gInterp_type b) 
+  | ser_pair a b => liftM2 pair (gInterp_type a) (gInterp_type b)
   | ser_list a => listOf (gInterp_type a)
   end.
 
@@ -428,36 +449,36 @@ Definition gSerializedValueSized (n : nat): G SerializedValue :=
 
 Instance genSerializedValueSized : GenSized SerializedValue :=
 {|
-  arbitrarySized := gSerializedValueSized 
+  arbitrarySized := gSerializedValueSized
 |}.
 
 (* Utils for QuickChick *)
 
 (* Helper functions when we want to state a property forAll x y z ... (someProp x y z ...) in QuickChick *)
 (* Where the generator for y depends on x, the generator for z depends on y, etc. *)
-Definition forAll2 {A B prop : Type} 
-                  `{Checkable prop} 
-                  `{Show A} 
-                  `{Show B} 
+Definition forAll2 {A B prop : Type}
+                  `{Checkable prop}
+                  `{Show A}
+                  `{Show B}
                    (genA : G A)
                    (fgenB : A -> G B)
                    (pf : A -> B -> prop) :=
   forAll genA (fun a => forAll (fgenB a) (fun b => pf a b)).
 
-Definition forAll3 {A B C prop : Type} 
-                  `{Checkable prop} 
-                  `{Show A} 
-                  `{Show B} 
-                  `{Show C} 
+Definition forAll3 {A B C prop : Type}
+                  `{Checkable prop}
+                  `{Show A}
+                  `{Show B}
+                  `{Show C}
                    (genA : G A)
                    (fgenB : A -> G B)
                    (fgenC : A -> B -> G C)
                    (pf : A -> B -> C -> prop) :=
-  forAll 
-    genA 
-    (fun a => 
-  forAll 
-    (fgenB a) 
+  forAll
+    genA
+    (fun a =>
+  forAll
+    (fgenB a)
   (fun b =>
   forAll
     (fgenC a b)
@@ -465,8 +486,8 @@ Definition forAll3 {A B C prop : Type}
 
 
 (* Little helper to avoid having to write out matches with "false ==> true" in None case all the time *)
-Definition isSomeCheck {A B : Type} `{Checkable B} (a : option A) (f : A -> B) : Checker := 
-match a with 
+Definition isSomeCheck {A B : Type} `{Checkable B} (a : option A) (f : A -> B) : Checker :=
+match a with
   | Some v => checker (f v)
   | None => false ==> true
 end.
@@ -474,24 +495,24 @@ end.
 (* A shallow way of embedding 'exists' in QC. Currently not very general, since we cant properly nest existPs
    because the predicate function returns a bool, and not a Checker. Need to review if this is even possible. *)
 Local Open Scope string_scope.
-Definition existsP {A prop : Type} 
-                  `{Checkable prop} 
-                  `{Show A} 
-                   (g : G A) 
-                   (p : A -> bool) := 
-  expectFailure (forAll g 
-  (fun a => whenFail ("Success - found witness satisfying the predicate!" ) 
+Definition existsP {A prop : Type}
+                  `{Checkable prop}
+                  `{Show A}
+                   (g : G A)
+                   (p : A -> bool) :=
+  expectFailure (forAll g
+  (fun a => whenFail ("Success - found witness satisfying the predicate!" )
     (negb (p a)))).
 
-Definition existsPShrink 
-                   {A prop : Type} 
-                  `{Checkable prop} 
+Definition existsPShrink
+                   {A prop : Type}
+                  `{Checkable prop}
                   `{Show A}
                   `{Shrink A}
-                   (g : G A) 
-                   (p : A -> bool) := 
-  expectFailure (forAllShrink g shrink 
-  (fun a => whenFail ("Success - found witness satisfying the predicate!" ) 
+                   (g : G A)
+                   (p : A -> bool) :=
+  expectFailure (forAllShrink g shrink
+  (fun a => whenFail ("Success - found witness satisfying the predicate!" )
     (negb (p a)))).
 
 (* QuickChick (
@@ -509,7 +530,7 @@ Success - found witness satisfying the predicate!
 (* QuickChick (
   existsPShrink arbitrary (fun (l : list nat) => 5 <? fold_left plus l 0 )
 ). *)
-(* 
+(*
 coqtop-stdout:[4; 2]
 Success - found witness satisfying the predicate!
 +++ Failed (as expected) after 5 tests and 3 shrinks. (0 discards)
@@ -517,9 +538,9 @@ Success - found witness satisfying the predicate!
 
 Definition conjoin_map {A prop : Type}
                       `{Checkable prop}
-                       (f : A -> prop) 
+                       (f : A -> prop)
                        (l : list A) := conjoin (map (checker o f) l).
-  
+
 Definition forEachMapEntry {A B prop : Type}
                           `{countable.Countable A}
                           `{base.EqDecision A}
@@ -527,12 +548,12 @@ Definition forEachMapEntry {A B prop : Type}
                            (m : FMap A B)
                            (pf : A -> B -> prop)
                            : Checker :=
-  let pf_ p := pf (fst p) (snd p) in 
+  let pf_ p := pf (fst p) (snd p) in
   conjoin_map pf_ (FMap.elements m).
 
 (* Repeats a generator for each element in the given list *)
 Fixpoint repeatWith {A prop : Type}
-                   `{Checkable prop} 
+                   `{Checkable prop}
                     (l : list A)
                     (c : A -> prop)
                     := conjoin (map (checker o c) l).
